Slight modification in one-op lemma

interface/App_alpha_map.fsti
@@ -5,27 +5,27 @@ module M = Map_extended
 
 open FStar.Seq
 
-//concrete state type of simpler MRDT
-val concrete_st_s : Type0
+//concrete state type of value MRDT
+val concrete_st_v : Type0
   
 // the concrete state type of map
-let concrete_st = M.t string concrete_st_s
+let concrete_st = M.t string concrete_st_v
 
-//concrete state type of simpler MRDT
-val init_st_s : concrete_st_s
+//concrete state type of value MRDT
+val init_st_v : concrete_st_v
 
 // init state of map
-let init_st = M.const init_st_s
+let init_st = M.const init_st_v
 
 let sel (s:concrete_st) (k:string) =
-  if M.contains s k then M.sel s k else init_st_s
+  if M.contains s k then M.sel s k else init_st_v
 
-//equivalence between 2 states of simpler MRDT
-let eq_s (s1 s2:concrete_st_s) : Type0 = s1 == s2
+//equivalence between 2 states of value MRDT
+let eq_v (s1 s2:concrete_st_v) : Type0 = s1 == s2
 
 // equivalence between 2 concrete states
 let eq (s1 s2:concrete_st) =
-  (forall k. (M.contains s1 k = M.contains s2 k) /\ eq_s (sel s1 k) (sel s2 k))
+ (forall k. (M.contains s1 k = M.contains s2 k) /\ eq_v (sel s1 k) (sel s2 k))
 
 let symmetric (a b:concrete_st) 
   : Lemma (requires eq a b)
@@ -39,14 +39,14 @@ let eq_is_equiv (a b:concrete_st)
   : Lemma (requires a == b)
           (ensures eq a b) = ()
 
-//operation type of simpler MRDT
-val app_op_s : eqtype 
+//operation type of value MRDT
+val app_op_v : eqtype 
 
-// operation type
+// operation type of map
 type app_op_t =
-  |Set : string (*key*) -> app_op_s -> app_op_t 
+  |Set : string (*key*) -> app_op_v -> app_op_t 
 
-type op_s = pos (*timestamp*) & (nat (*replica ID*) & app_op_s)
+type op_v = pos (*timestamp*) & (nat (*replica ID*) & app_op_v)
 
 type op_t = pos (*timestamp*) & (nat (*replica ID*) & app_op_t)
 
@@ -56,11 +56,11 @@ let distinct_ops (ts1,_) (ts2,_) = ts1 =!= ts2
 
 type log = seq op_t
 
-//do function of simpler MRDT
-val do_s (s:concrete_st_s) (o:op_s) : concrete_st_s
+//do function of value MRDT
+val do_v (s:concrete_st_v) (o:op_v) : concrete_st_v
 
-//convert map operation to simpler MRDT operation
-let get_op_s (o:op_t) : op_s =
+//convert map operation to value MRDT operation
+let get_op_v (o:op_t) : op_v =
   match o with
   |ts, (rid, Set _ o) -> (ts,(rid,o))
 
@@ -69,8 +69,11 @@ let get_key (_,(_,Set k _)) = k
 // apply an operation to a state
 let do (s:concrete_st) (o:op_t) : concrete_st =
   let k = get_key o in
-  M.upd s k (do_s (sel s k) (get_op_s o))
+  M.upd s k (do_v (sel s k) (get_op_v o))
 
+let commutes_with_v (o1 o2:op_v) =
+  forall s. eq_v (do_v (do_v s o1) o2) (do_v (do_v s o2) o1)
+  
 let commutes_with (o1 o2:op_t) =
   forall s. eq (do (do s o1) o2) (do (do s o2) o1)
 
@@ -86,96 +89,101 @@ type rc_res =
   |Snd_then_fst //o2 -> o1
   |Either
 
-//conflict resolution of simpler MRDT
-val rc_s (o1 o2:op_s) : rc_res
+//conflict resolution of value MRDT
+val rc_v (o1 o2:op_v) : rc_res
 
 //conflict resolution of map
 let rc (o1 o2:op_t) : rc_res = 
-  if get_key o1 = get_key o2 then rc_s (get_op_s o1) (get_op_s o2) else Either
+  if get_key o1 = get_key o2 then rc_v (get_op_v o1) (get_op_v o2) else Either
 
 //three-way merge of simpler MRDT
-val merge_s (l a b:concrete_st_s) : concrete_st_s
+val merge_v (l a b:concrete_st_v) : concrete_st_v
 
 // concrete merge operation of map
 let merge (l a b:concrete_st) : concrete_st =
   let eles = S.union (M.domain l) (S.union (M.domain a) (M.domain b)) in
-  let u = M.const_on eles init_st_s in
-  M.iter_upd (fun k v -> merge_s (sel l k) (sel a k) (sel b k)) u
-
+  let u = M.const_on eles init_st_v in
+  M.iter_upd (fun k v -> merge_v (sel l k) (sel a k) (sel b k)) u 
+  
 /////////////////////////////////////////////////////////////////////////////
 
 val rc_non_comm (o1 o2:op_t)
   : Lemma (requires distinct_ops o1 o2)
-          (ensures Either? (rc o1 o2) <==> commutes_with o1 o2)
-
+          (ensures Either? (rc o1 o2) <==> commutes_with o1 o2) 
+          
 val no_rc_chain (o1 o2 o3:op_t)
   : Lemma (requires distinct_ops o1 o2 /\ distinct_ops o2 o3)
           (ensures ~ (Fst_then_snd? (rc o1 o2) /\ Fst_then_snd? (rc o2 o3)))
 
-val cond_comm_base (s:concrete_st) (o1 o2:op_t) (o3:op_t{distinct_ops o1 o2 /\ distinct_ops o1 o3 /\ distinct_ops o2 o3})
-    : (b:bool{(Fst_then_snd? (rc o1 o2) /\ ~ (Either? (rc o2 o3))) ==> eq (do (do (do s o1) o2) o3) (do (do (do s o2) o1) o3)})
+val cond_comm_base (s:concrete_st) (o1 o2 o3:op_t) 
+  : Lemma (requires distinct_ops o1 o2 /\ distinct_ops o2 o3 /\ distinct_ops o1 o3 /\
+                    Fst_then_snd? (rc o1 o2) /\ ~ (Either? (rc o2 o3)))
+          (ensures eq (do (do (do s o1) o2) o3) (do (do (do s o2) o1) o3))
 
 val cond_comm_ind (s:concrete_st) (o1 o2 o3 o:op_t) (l:seq op_t)
-  : Lemma (requires distinct_ops o1 o2 /\ distinct_ops o1 o3 /\ distinct_ops o2 o3 /\ cond_comm_base s o1 o2 o3 /\
+  : Lemma (requires distinct_ops o1 o2 /\ distinct_ops o1 o3 /\ distinct_ops o2 o3 /\ 
+                    Fst_then_snd? (rc o1 o2) /\ ~ (Either? (rc o2 o3)) /\
                     eq (do (apply_log (do (do s o1) o2) l) o3) (do (apply_log (do (do s o2) o1) l) o3))
           (ensures eq (do (do (apply_log (do (do s o1) o2) l) o) o3) (do (do (apply_log (do (do s o2) o1) l) o) o3))
                   
 ////////////////////////////////////////////////////////////////////////////
 
 //merge is commutative
-val merge_comm (l a b:concrete_st)
-  : Lemma (ensures (eq (merge l a b) (merge l b a)))
+val merge_comm_v (l a b: concrete_st_v) 
+  : Lemma (ensures eq_v (merge_v l a b) (merge_v l b a))
+          [SMTPat (merge_v l a b)]
+ 
+let merge_comm (l a b:concrete_st)
+  : Lemma (ensures (eq (merge l a b) (merge l b a))) = ()
 
 //merge is idempotent
-val merge_idem (s:concrete_st)
-  : Lemma (ensures eq (merge s s s) s)
+val merge_idem_v (s: concrete_st_v) 
+  : Lemma (ensures eq_v (merge_v s s s) s)
+          [SMTPat (merge_v s s s)]
+          
+let merge_idem (s:concrete_st)
+  : Lemma (ensures eq (merge s s s) s) = ()
 
-////////////////////////////////////////////////////////////////////////////
-
-//helper lemmas
-val lemma_do (s:concrete_st) (o:op_t)
-  : Lemma (ensures (forall k. k = get_key o ==> eq_s (sel (do s o) k) (do_s (sel s k) (get_op_s o))))
-
-val lemma_merge (l a b:concrete_st)
-  : Lemma (ensures (forall k. eq_s (sel (merge l a b) k) (merge_s (sel l k) (sel a k) (sel b k))) )
+//////////////////////////////////////////////////////////////////////////
 
 (*Two OP RC*)
 //////////////// 
-val rc_ind_right_s (l a b:concrete_st_s) (o1 o2 o2':op_s) 
-  : Lemma (requires rc_s o1 o2 <> Either /\ distinct_ops o1 o2 /\ distinct_ops o1 o2' /\ distinct_ops o2 o2' /\ 
-                    eq_s (merge_s l (do_s a o1) (do_s b o2)) (do_s (merge_s l (do_s a o1) b) o2))
-          (ensures eq_s (merge_s l (do_s a o1) (do_s (do_s b o2') o2)) (do_s (merge_s l (do_s a o1) (do_s b o2')) o2))
+val rc_ind_right_v (l a b:concrete_st_v) (o1 o2 o2':op_v) 
+  : Lemma (requires Fst_then_snd? (rc_v o1 o2) /\
+                    distinct_ops o1 o2 /\ distinct_ops o1 o2' /\ distinct_ops o2 o2' /\  
+                    eq_v (merge_v l (do_v a o1) (do_v b o2)) (do_v (merge_v l (do_v a o1) b) o2))
+          (ensures eq_v (merge_v l (do_v a o1) (do_v (do_v b o2') o2)) (do_v (merge_v l (do_v a o1) (do_v b o2')) o2))
 
-val rc_ind_right_ne (l a b:concrete_st) (o1 o2 o2':op_t)
+let rc_ind_right_ne (l a b:concrete_st) (o1 o2 o2':op_t)
   : Lemma (requires Fst_then_snd? (rc o1 o2) /\
                     distinct_ops o1 o2 /\ distinct_ops o1 o2' /\ distinct_ops o2 o2' /\  
-                    ~ (get_key o1 = get_key o2 /\ get_key o2 = get_key o2') /\
+                    ~ (get_key o2 = get_key o2' /\ Fst_then_snd? (rc_v (get_op_v o1) (get_op_v o2))) /\
                     eq (merge l (do a o1) (do b o2)) (do (merge l (do a o1) b) o2))
-          (ensures eq (merge l (do a o1) (do (do b o2') o2)) (do (merge l (do a o1) (do b o2')) o2))
+          (ensures eq (merge l (do a o1) (do (do b o2') o2)) (do (merge l (do a o1) (do b o2')) o2)) = ()                
 
 let rc_ind_right (l a b:concrete_st) (o1 o2 o2':op_t)
   : Lemma (requires Fst_then_snd? (rc o1 o2) /\
                     distinct_ops o1 o2 /\ distinct_ops o1 o2' /\ distinct_ops o2 o2' /\  
                     eq (merge l (do a o1) (do b o2)) (do (merge l (do a o1) b) o2))
           (ensures eq (merge l (do a o1) (do (do b o2') o2)) (do (merge l (do a o1) (do b o2')) o2)) =
-  assert (rc_s (get_op_s o1) (get_op_s o2) <> Either);
   let k = get_key o2' in
   let l' = sel l k in let a' = sel a k in let b' = sel b k in 
-  if get_key o2 = get_key o1 && get_key o1 = k then 
-    rc_ind_right_s l' a' b' (get_op_s o1) (get_op_s o2) (get_op_s o2')
+  if get_key o2 = k && Fst_then_snd? (rc_v (get_op_v o1) (get_op_v o2)) then 
+    rc_ind_right_v l' a' b' (get_op_v o1) (get_op_v o2) (get_op_v o2')
   else rc_ind_right_ne l a b o1 o2 o2'
 
-val rc_ind_left_s (l a b:concrete_st_s) (o1 o2 o1':op_s)
-  : Lemma (requires rc_s o1 o2 <> Either /\ distinct_ops o1 o2 /\ distinct_ops o1 o1' /\ distinct_ops o2 o1' /\  
-                    eq_s (merge_s l (do_s a o1) (do_s b o2)) (do_s (merge_s l (do_s a o1) b) o2))
-          (ensures eq_s (merge_s l (do_s (do_s a o1') o1) (do_s b o2)) (do_s (merge_s l (do_s (do_s a o1') o1) b) o2))
+val rc_ind_left_v (l a b:concrete_st_v) (o1 o2 o1':op_v)
+  : Lemma (requires Fst_then_snd? (rc_v o1 o2) /\ 
+                    distinct_ops o1 o2 /\ distinct_ops o1 o1' /\ distinct_ops o2 o1' /\  
+                    eq_v (merge_v l (do_v a o1) (do_v b o2)) (do_v (merge_v l (do_v a o1) b) o2))
+          (ensures eq_v (merge_v l (do_v (do_v a o1') o1) (do_v b o2)) (do_v (merge_v l (do_v (do_v a o1') o1) b) o2))
 
-val rc_ind_left_ne (l a b:concrete_st) (o1 o2 o1':op_t)
+let rc_ind_left_ne (l a b:concrete_st) (o1 o2 o1':op_t)
   : Lemma (requires Fst_then_snd? (rc o1 o2) /\
                     distinct_ops o1 o2 /\ distinct_ops o1 o1' /\ distinct_ops o2 o1' /\  
-                    ~ (get_key o1 = get_key o2 /\ get_key o2 = get_key o1') /\
+                    ~ (get_key o1 = get_key o1' /\ Fst_then_snd? (rc_v (get_op_v o1) (get_op_v o2))) /\
                     eq (merge l (do a o1) (do b o2)) (do (merge l (do a o1) b) o2))
-          (ensures eq (merge l (do (do a o1') o1) (do b o2)) (do (merge l (do (do a o1') o1) b) o2))
+          (ensures eq (merge l (do (do a o1') o1) (do b o2)) (do (merge l (do (do a o1') o1) b) o2)) = ()
           
 let rc_ind_left (l a b:concrete_st) (o1 o2 o1':op_t)
   : Lemma (requires Fst_then_snd? (rc o1 o2) /\
@@ -184,21 +192,22 @@ let rc_ind_left (l a b:concrete_st) (o1 o2 o1':op_t)
           (ensures eq (merge l (do (do a o1') o1) (do b o2)) (do (merge l (do (do a o1') o1) b) o2)) =
   let k = get_key o1' in
   let l' = sel l k in let a' = sel a k in let b' = sel b k in 
-  if get_key o2 = get_key o1 && get_key o1 = k then 
-    rc_ind_left_s l' a' b' (get_op_s o1) (get_op_s o2) (get_op_s o1')
+  if get_key o1 = k && Fst_then_snd? (rc_v (get_op_v o1) (get_op_v o2)) then 
+    rc_ind_left_v l' a' b' (get_op_v o1) (get_op_v o2) (get_op_v o1')
   else rc_ind_left_ne l a b o1 o2 o1'
 
-val rc_ind_lca_s (l:concrete_st_s) (o1 o2 o:op_s)
-  : Lemma (requires rc_s o1 o2 <> Either /\ distinct_ops o1 o2 /\ distinct_ops o o1 /\ distinct_ops o o2 /\
-                    eq_s (merge_s l (do_s l o1) (do_s l o2)) (do_s (do_s l o1) o2))
-          (ensures eq_s (merge_s (do_s l o) (do_s (do_s l o) o1) (do_s (do_s l o) o2)) (do_s (do_s (do_s l o) o1) o2))
+val rc_ind_lca_v (l:concrete_st_v) (o1 o2 o:op_v)
+  : Lemma (requires Fst_then_snd? (rc_v o1 o2) /\
+                    distinct_ops o1 o2 /\ distinct_ops o o1 /\ distinct_ops o o2 /\
+                    eq_v (merge_v l (do_v l o1) (do_v l o2)) (do_v (do_v l o1) o2))
+          (ensures eq_v (merge_v (do_v l o) (do_v (do_v l o) o1) (do_v (do_v l o) o2)) (do_v (do_v (do_v l o) o1) o2))
 
-val rc_ind_lca_ne (l:concrete_st) (o1 o2 o:op_t)
+let rc_ind_lca_ne (l:concrete_st) (o1 o2 o:op_t)
   : Lemma (requires Fst_then_snd? (rc o1 o2) /\ 
                     distinct_ops o1 o2 /\ distinct_ops o1 o /\ distinct_ops o o2 /\
-                    ~ (get_key o1 = get_key o2 /\ get_key o2 = get_key o) /\
+                    ~ (get_key o1 = get_key o /\ Fst_then_snd? (rc_v (get_op_v o1) (get_op_v o2))) /\
                     eq (merge l (do l o1) (do l o2)) (do (do l o1) o2))
-          (ensures eq (merge (do l o) (do (do l o) o1) (do (do l o) o2)) (do (do (do l o) o1) o2))
+          (ensures eq (merge (do l o) (do (do l o) o1) (do (do l o) o2)) (do (do (do l o) o1) o2)) = ()
           
 //Special case of rc_intermediate_v1
 let rc_ind_lca (l:concrete_st) (o1 o2 o:op_t)
@@ -208,26 +217,26 @@ let rc_ind_lca (l:concrete_st) (o1 o2 o:op_t)
           (ensures eq (merge (do l o) (do (do l o) o1) (do (do l o) o2)) (do (do (do l o) o1) o2)) =
   let k = get_key o in
   let l' = sel l k in
-  if get_key o2 = get_key o1 && get_key o1 = k then 
-    rc_ind_lca_s l' (get_op_s o1) (get_op_s o2) (get_op_s o)
+  if get_key o1 = k && Fst_then_snd? (rc_v (get_op_v o1) (get_op_v o2)) then 
+    rc_ind_lca_v l' (get_op_v o1) (get_op_v o2) (get_op_v o)
   else rc_ind_lca_ne l o1 o2 o
           
 val rc_base (o1 o2:op_t)
   : Lemma (requires Fst_then_snd? (rc o1 o2) /\ distinct_ops o1 o2)
           (ensures eq (merge init_st (do init_st o1) (do init_st o2)) (do (do init_st o1) o2))
 
-val rc_inter_base_right_s (l a b c:concrete_st_s) (o1 o2 ob ol:op_s)
-  : Lemma (requires rc_s o1 o2 <> Either /\ rc_s ob ol <> Either /\ 
+val rc_inter_base_right_v (l a b c:concrete_st_v) (o1 o2 ob ol:op_v)
+  : Lemma (requires Fst_then_snd? (rc_v o1 o2) /\ Fst_then_snd? (rc_v ob ol) /\
                     distinct_ops o1 o2 /\ distinct_ops o1 ob /\ distinct_ops o1 ol /\ distinct_ops o2 ob /\ distinct_ops o2 ol /\ distinct_ops ob ol /\ 
-                    eq_s (merge_s (do_s l ol) (do_s (do_s a ol) o1) (do_s (do_s b ol) o2)) (do_s (do_s (do_s c ol) o1) o2) /\
-                    eq_s (merge_s l (do_s a o1) (do_s b o2)) (do_s (do_s c o1) o2) /\
-                    eq_s (merge_s l (do_s a ol) (do_s b ob)) (do_s (do_s c ob) ol)) //***EXTRA***
-          (ensures eq_s (merge_s (do_s l ol) (do_s (do_s a ol) o1) (do_s (do_s (do_s b ob) ol) o2)) (do_s (do_s (do_s (do_s c ob) ol) o1) o2))
+                    eq_v (merge_v (do_v l ol) (do_v (do_v a ol) o1) (do_v (do_v b ol) o2)) (do_v (do_v (do_v c ol) o1) o2) /\
+                    eq_v (merge_v l (do_v a o1) (do_v b o2)) (do_v (do_v c o1) o2) /\
+                    eq_v (merge_v l (do_v a ol) (do_v b ob)) (do_v (do_v c ob) ol)) //***EXTRA***
+          (ensures eq_v (merge_v (do_v l ol) (do_v (do_v a ol) o1) (do_v (do_v (do_v b ob) ol) o2)) (do_v (do_v (do_v (do_v c ob) ol) o1) o2))
 
 val rc_inter_base_right_ne (l a b c:concrete_st) (o1 o2 ob ol:op_t) 
   : Lemma (requires Fst_then_snd? (rc o1 o2) /\ Fst_then_snd? (rc ob ol) /\ 
                     distinct_ops o1 o2 /\ distinct_ops o1 ob /\ distinct_ops o1 ol /\ distinct_ops o2 ob /\ distinct_ops o2 ol /\ distinct_ops ob ol /\ 
-                    ~ (get_key o1 = get_key o2 /\ get_key o2 = get_key ob) /\
+                    ~ (get_key o2 = get_key ob /\ Fst_then_snd? (rc_v (get_op_v o1) (get_op_v o2)) /\ Fst_then_snd? (rc_v (get_op_v ob) (get_op_v ol))) /\
                     eq (merge (do l ol) (do (do a ol) o1) (do (do b ol) o2)) (do (do (do c ol) o1) o2) /\
                     eq (merge l (do a o1) (do b o2)) (do (do c o1) o2) /\
                     eq (merge l (do a ol) (do b ob)) (do (do c ob) ol)) //***EXTRA***
@@ -242,22 +251,22 @@ let rc_inter_base_right (l a b c:concrete_st) (o1 o2 ob ol:op_t)
           (ensures eq (merge (do l ol) (do (do a ol) o1) (do (do (do b ob) ol) o2)) (do (do (do (do c ob) ol) o1) o2)) =
   let k = get_key ob in
   let l' = sel l k in let a' = sel a k in let b' = sel b k in let c' = sel c k in
-  if get_key o2 = get_key o1 && get_key o1 = k then 
-    rc_inter_base_right_s l' a' b' c' (get_op_s o1) (get_op_s o2) (get_op_s ob) (get_op_s ol)
+  if get_key o2 = k && Fst_then_snd? (rc_v (get_op_v o1) (get_op_v o2)) && Fst_then_snd? (rc_v (get_op_v ob) (get_op_v ol)) then 
+    rc_inter_base_right_v l' a' b' c' (get_op_v o1) (get_op_v o2) (get_op_v ob) (get_op_v ol)
   else rc_inter_base_right_ne l a b c o1 o2 ob ol
 
-val rc_inter_base_left_s (l a b c:concrete_st_s) (o1 o2 ob ol:op_s)
-  : Lemma (requires rc_s o1 o2 <> Either /\ rc_s ob ol <> Either /\ 
+val rc_inter_base_left_v (l a b c:concrete_st_v) (o1 o2 ob ol:op_v)
+  : Lemma (requires Fst_then_snd? (rc_v o1 o2) /\ Fst_then_snd? (rc_v ob ol) /\
                     distinct_ops o1 o2 /\ distinct_ops o1 ob /\ distinct_ops o1 ol /\ distinct_ops o2 ob /\ distinct_ops o2 ol /\ distinct_ops ob ol /\ 
-                    eq_s (merge_s (do_s l ol) (do_s (do_s a ol) o1) (do_s (do_s b ol) o2)) (do_s (do_s (do_s c ol) o1) o2) /\
-                    eq_s (merge_s l (do_s a o1) (do_s b o2)) (do_s (do_s c o1) o2) /\
-                    eq_s (merge_s l (do_s a ob) (do_s b ol)) (do_s (do_s c ob) ol)) //***EXTRA***
-          (ensures eq_s (merge_s (do_s l ol) (do_s (do_s (do_s a ob) ol) o1) (do_s (do_s b ol) o2)) (do_s (do_s (do_s (do_s c ob) ol) o1) o2))
+                    eq_v (merge_v (do_v l ol) (do_v (do_v a ol) o1) (do_v (do_v b ol) o2)) (do_v (do_v (do_v c ol) o1) o2) /\
+                    eq_v (merge_v l (do_v a o1) (do_v b o2)) (do_v (do_v c o1) o2) /\
+                    eq_v (merge_v l (do_v a ob) (do_v b ol)) (do_v (do_v c ob) ol)) //***EXTRA***
+          (ensures eq_v (merge_v (do_v l ol) (do_v (do_v (do_v a ob) ol) o1) (do_v (do_v b ol) o2)) (do_v (do_v (do_v (do_v c ob) ol) o1) o2))
 
 val rc_inter_base_left_ne (l a b c:concrete_st) (o1 o2 ob ol:op_t) 
   : Lemma (requires Fst_then_snd? (rc o1 o2) /\ Fst_then_snd? (rc ob ol) /\ 
                     distinct_ops o1 o2 /\ distinct_ops o1 ob /\ distinct_ops o1 ol /\ distinct_ops o2 ob /\ distinct_ops o2 ol /\ distinct_ops ob ol /\ 
-                    ~ (get_key o1 = get_key o2 /\ get_key o2 = get_key ob) /\
+                    ~ (get_key o1 = get_key ob /\ Fst_then_snd? (rc_v (get_op_v o1) (get_op_v o2)) /\ Fst_then_snd? (rc_v (get_op_v ob) (get_op_v ol))) /\
                     eq (merge (do l ol) (do (do a ol) o1) (do (do b ol) o2)) (do (do (do c ol) o1) o2) /\
                     eq (merge l (do a o1) (do b o2)) (do (do c o1) o2) /\
                     eq (merge l (do a ob) (do b ol)) (do (do c ob) ol)) //***EXTRA***
@@ -272,23 +281,24 @@ let rc_inter_base_left (l a b c:concrete_st) (o1 o2 ob ol:op_t)
           (ensures eq (merge (do l ol) (do (do (do a ob) ol) o1) (do (do b ol) o2)) (do (do (do (do c ob) ol) o1) o2)) =
   let k = get_key ob in
   let l' = sel l k in let a' = sel a k in let b' = sel b k in let c' = sel c k in
-  if get_key o2 = get_key o1 && get_key o1 = k then 
-    rc_inter_base_left_s l' a' b' c' (get_op_s o1) (get_op_s o2) (get_op_s ob) (get_op_s ol)
+  if get_key o1 = k && Fst_then_snd? (rc_v (get_op_v o1) (get_op_v o2)) && Fst_then_snd? (rc_v (get_op_v ob) (get_op_v ol)) then 
+    rc_inter_base_left_v l' a' b' c' (get_op_v o1) (get_op_v o2) (get_op_v ob) (get_op_v ol)
   else rc_inter_base_left_ne l a b c o1 o2 ob ol
 
-val rc_inter_right_s (l a b c:concrete_st_s) (o1 o2 ob ol o:op_s)
-  : Lemma (requires rc_s o1 o2 <> Either /\ rc_s ob ol <> Either /\ 
+val rc_inter_right_v (l a b c:concrete_st_v) (o1 o2 ob ol o:op_v)
+  : Lemma (requires Fst_then_snd? (rc_v o1 o2) /\ Fst_then_snd? (rc_v ob ol) /\
                     distinct_ops o1 o2 /\ distinct_ops o1 ob /\ distinct_ops o1 ol /\ distinct_ops o1 o /\ distinct_ops o2 ob /\ 
                     distinct_ops o2 ol /\ distinct_ops o2 o /\ distinct_ops ob ol /\ distinct_ops ob o /\ distinct_ops ol o /\
                     get_rid o <> get_rid ol /\
-                    eq_s (merge_s (do_s l ol) (do_s (do_s a ol) o1) (do_s (do_s (do_s b ob) ol) o2)) (do_s (do_s (do_s (do_s c ob) ol) o1) o2))
-      (ensures eq_s (merge_s (do_s l ol) (do_s (do_s a ol) o1) (do_s (do_s (do_s (do_s b o) ob) ol) o2)) (do_s (do_s (do_s (do_s (do_s c o) ob) ol) o1) o2))
+                    ((~ (commutes_with_v o ob)) \/ Fst_then_snd? (rc_v o ol)) /\
+                    eq_v (merge_v (do_v l ol) (do_v (do_v a ol) o1) (do_v (do_v (do_v b ob) ol) o2)) (do_v (do_v (do_v (do_v c ob) ol) o1) o2))
+      (ensures eq_v (merge_v (do_v l ol) (do_v (do_v a ol) o1) (do_v (do_v (do_v (do_v b o) ob) ol) o2)) (do_v (do_v (do_v (do_v (do_v c o) ob) ol) o1) o2))
 
 val rc_inter_right_ne (l a b c:concrete_st) (o1 o2 ob ol o:op_t) 
   : Lemma (requires Fst_then_snd? (rc o1 o2) /\ Fst_then_snd? (rc ob ol) /\ 
                     distinct_ops o1 o2 /\ distinct_ops o1 ob /\ distinct_ops o1 ol /\ distinct_ops o1 o /\ distinct_ops o2 ob /\ 
                     distinct_ops o2 ol /\ distinct_ops o2 o /\ distinct_ops ob ol /\ distinct_ops ob o /\ distinct_ops ol o /\
-                    ~ (get_key o1 = get_key o2 /\ get_key o2 = get_key ob) /\
+                    ~ (get_key o2 = get_key ob /\ Fst_then_snd? (rc_v (get_op_v o1) (get_op_v o2)) /\ Fst_then_snd? (rc_v (get_op_v ob) (get_op_v ol))) /\
                     get_rid o <> get_rid ol (*o,ol must be concurrent*) /\
                     ((~ (commutes_with o ob)) \/ Fst_then_snd? (rc o ol)) /\
                     eq (merge (do l ol) (do (do a ol) o1) (do (do (do b ob) ol) o2)) (do (do (do (do c ob) ol) o1) o2))
@@ -304,23 +314,24 @@ let rc_inter_right (l a b c:concrete_st) (o1 o2 ob ol o:op_t)
       (ensures eq (merge (do l ol) (do (do a ol) o1) (do (do (do (do b o) ob) ol) o2)) (do (do (do (do (do c o) ob) ol) o1) o2)) =
   let k = get_key o in
   let l' = sel l k in let a' = sel a k in let b' = sel b k in let c' = sel c k in
-  if get_key o2 = get_key o1 && get_key o1 = k then 
-    rc_inter_right_s l' a' b' c' (get_op_s o1) (get_op_s o2) (get_op_s ob) (get_op_s ol) (get_op_s o)
+  if get_key o2 = k && Fst_then_snd? (rc_v (get_op_v o1) (get_op_v o2)) && Fst_then_snd? (rc_v (get_op_v ob) (get_op_v ol)) then 
+    rc_inter_right_v l' a' b' c' (get_op_v o1) (get_op_v o2) (get_op_v ob) (get_op_v ol) (get_op_v o)
   else rc_inter_right_ne l a b c o1 o2 ob ol o
 
-val rc_inter_left_s (l a b c:concrete_st_s) (o1 o2 ob ol o:op_s)
-  : Lemma (requires rc_s o1 o2 <> Either /\ rc_s ob ol <> Either /\ 
+val rc_inter_left_v (l a b c:concrete_st_v) (o1 o2 ob ol o:op_v)
+  : Lemma (requires Fst_then_snd? (rc_v o1 o2) /\ Fst_then_snd? (rc_v ob ol) /\
                     distinct_ops o1 o2 /\ distinct_ops o1 ob /\ distinct_ops o1 ol /\ distinct_ops o1 o /\ distinct_ops o2 ob /\ 
                     distinct_ops o2 ol /\ distinct_ops o2 o /\ distinct_ops ob ol /\ distinct_ops ob o /\ distinct_ops ol o /\
                     get_rid o <> get_rid ol /\
-                    eq_s (merge_s (do_s l ol) (do_s (do_s (do_s a ob) ol) o1) (do_s (do_s b ol) o2)) (do_s (do_s (do_s (do_s c ob) ol) o1) o2))
-      (ensures eq_s (merge_s (do_s l ol) (do_s (do_s (do_s (do_s a o) ob) ol) o1) (do_s (do_s b ol) o2)) (do_s (do_s (do_s (do_s (do_s c o) ob) ol) o1) o2))
+                    ((~ (commutes_with_v o ob)) \/ Fst_then_snd? (rc_v o ol)) /\
+                    eq_v (merge_v (do_v l ol) (do_v (do_v (do_v a ob) ol) o1) (do_v (do_v b ol) o2)) (do_v (do_v (do_v (do_v c ob) ol) o1) o2))
+      (ensures eq_v (merge_v (do_v l ol) (do_v (do_v (do_v (do_v a o) ob) ol) o1) (do_v (do_v b ol) o2)) (do_v (do_v (do_v (do_v (do_v c o) ob) ol) o1) o2))
 
 val rc_inter_left_ne (l a b c:concrete_st) (o1 o2 ob ol o:op_t) 
   : Lemma (requires Fst_then_snd? (rc o1 o2) /\ Fst_then_snd? (rc ob ol) /\ 
                     distinct_ops o1 o2 /\ distinct_ops o1 ob /\ distinct_ops o1 ol /\ distinct_ops o1 o /\ distinct_ops o2 ob /\ 
                     distinct_ops o2 ol /\ distinct_ops o2 o /\ distinct_ops ob ol /\ distinct_ops ob o /\ distinct_ops ol o /\
-                    ~ (get_key o1 = get_key o2 /\ get_key o2 = get_key ob) /\
+                    ~ (get_key o1 = get_key ob /\ Fst_then_snd? (rc_v (get_op_v o1) (get_op_v o2)) /\ Fst_then_snd? (rc_v (get_op_v ob) (get_op_v ol))) /\
                     get_rid o <> get_rid ol (*o,ol must be concurrent*) /\
                     ((~ (commutes_with o ob)) \/ Fst_then_snd? (rc o ol)) /\
                     eq (merge (do l ol) (do (do (do a ob) ol) o1) (do (do b ol) o2)) (do (do (do (do c ob) ol) o1) o2))
@@ -336,23 +347,24 @@ let rc_inter_left (l a b c:concrete_st) (o1 o2 ob ol o:op_t)
       (ensures eq (merge (do l ol) (do (do (do (do a o) ob) ol) o1) (do (do b ol) o2)) (do (do (do (do (do c o) ob) ol) o1) o2)) =
   let k = get_key o in
   let l' = sel l k in let a' = sel a k in let b' = sel b k in let c' = sel c k in
-  if get_key o2 = get_key o1 && get_key o1 = k then 
-    rc_inter_left_s l' a' b' c' (get_op_s o1) (get_op_s o2) (get_op_s ob) (get_op_s ol) (get_op_s o)
+  if get_key o1 = k && Fst_then_snd? (rc_v (get_op_v o1) (get_op_v o2)) && Fst_then_snd? (rc_v (get_op_v ob) (get_op_v ol)) then 
+    rc_inter_left_v l' a' b' c' (get_op_v o1) (get_op_v o2) (get_op_v ob) (get_op_v ol) (get_op_v o)
   else rc_inter_left_ne l a b c o1 o2 ob ol o
 
-val rc_inter_lca_s (l a b c:concrete_st_s) (o1 o2 ol oi:op_s)
-  : Lemma (requires rc_s o1 o2 <> Either /\ 
+//CHECK!!
+val rc_inter_lca_v (l a b c:concrete_st_v) (o1 o2 ol oi:op_v)
+  : Lemma (requires Fst_then_snd? (rc_v o1 o2) /\ 
                     distinct_ops o1 o2 /\ distinct_ops o1 ol /\ distinct_ops o1 oi /\ distinct_ops o2 ol /\ distinct_ops o2 oi /\ distinct_ops ol oi /\
-                    (exists o. rc_s o ol <> Either) /\ 
-                    (exists o. rc_s o oi <> Either) /\
-                    eq_s (merge_s (do_s l oi) (do_s (do_s a oi) o1) (do_s (do_s b oi) o2)) (do_s (do_s (do_s c oi) o1) o2) /\
-                    eq_s (merge_s (do_s l ol) (do_s (do_s a ol) o1) (do_s (do_s b ol) o2)) (do_s (do_s (do_s c ol) o1) o2))
-    (ensures eq_s (merge_s (do_s (do_s l oi) ol) (do_s (do_s (do_s a oi) ol) o1) (do_s (do_s (do_s b oi) ol) o2)) (do_s (do_s (do_s (do_s c oi) ol) o1) o2))
+                    (exists o. Fst_then_snd? (rc_v o ol)) /\ 
+                    (exists o. Fst_then_snd? (rc_v o oi)) /\
+                    eq_v (merge_v (do_v l oi) (do_v (do_v a oi) o1) (do_v (do_v b oi) o2)) (do_v (do_v (do_v c oi) o1) o2) /\
+                    eq_v (merge_v (do_v l ol) (do_v (do_v a ol) o1) (do_v (do_v b ol) o2)) (do_v (do_v (do_v c ol) o1) o2))
+    (ensures eq_v (merge_v (do_v (do_v l oi) ol) (do_v (do_v (do_v a oi) ol) o1) (do_v (do_v (do_v b oi) ol) o2)) (do_v (do_v (do_v (do_v c oi) ol) o1) o2))
 
 val rc_inter_lca_ne (l a b c:concrete_st) (o1 o2 ol oi:op_t) 
   : Lemma (requires Fst_then_snd? (rc o1 o2) /\ 
                     distinct_ops o1 o2 /\ distinct_ops o1 ol /\ distinct_ops o1 oi /\ distinct_ops o2 ol /\ distinct_ops o2 oi /\ distinct_ops ol oi /\
-                    ~ (get_key o1 = get_key o2 /\ get_key o1 = get_key oi /\ get_key o1 = get_key ol) /\
+                    ~ (get_key o1 = get_key o2 /\ get_key o1 = get_key oi /\ get_key o1 = get_key ol /\ Fst_then_snd? (rc_v (get_op_v o1) (get_op_v o2))) /\
                     
                     (exists o. Fst_then_snd? (rc o ol)) /\ 
                     (exists o. Fst_then_snd? (rc o oi)) /\ 
@@ -372,63 +384,61 @@ let rc_inter_lca (l a b c:concrete_st) (o1 o2 ol oi:op_t)
   let k = get_key oi in
   let l' = sel l k in let a' = sel a k in let b' = sel b k in let c' = sel c k in
   if get_key o2 = get_key o1 && get_key o1 = k && get_key o1 = get_key ol then 
-    rc_inter_lca_s l' a' b' c' (get_op_s o1) (get_op_s o2) (get_op_s ol) (get_op_s oi)
+    rc_inter_lca_v l' a' b' c' (get_op_v o1) (get_op_v o2) (get_op_v ol) (get_op_v oi)
   else rc_inter_lca_ne l a b c o1 o2 ol oi
 
 (*One op*)
 ///////////////
-val one_op_ind_right_s (l a b:concrete_st_s) (o2 o2':op_s) 
+val one_op_ind_right_v (l a b:concrete_st_v) (o2 o2':op_v) 
   : Lemma (requires distinct_ops o2 o2' /\ 
-                    eq_s (merge_s l a (do_s b o2)) (do_s (merge_s l a b) o2))
-           (ensures eq_s (merge_s l a (do_s (do_s b o2') o2)) (do_s (merge_s l a (do_s b o2')) o2))
+                    eq_v (merge_v l a (do_v b o2)) (do_v (merge_v l a b) o2))
+           (ensures eq_v (merge_v l a (do_v (do_v b o2') o2)) (do_v (merge_v l a (do_v b o2')) o2))
 
-val one_op_ind_right_ne (l a b:concrete_st) (o2 o2':op_t)
+let one_op_ind_right_ne (l a b:concrete_st) (o2 o2':op_t)
   : Lemma (requires distinct_ops o2 o2' /\ 
                     ~ (get_key o2 = get_key o2') /\
                     eq (merge l a (do b o2)) (do (merge l a b) o2))
-           (ensures eq (merge l a (do (do b o2') o2)) (do (merge l a (do b o2')) o2))
+           (ensures eq (merge l a (do (do b o2') o2)) (do (merge l a (do b o2')) o2)) = ()
 
 let one_op_ind_right (l a b:concrete_st) (o2 o2':op_t)
    : Lemma (requires distinct_ops o2 o2' /\ eq (merge l a (do b o2)) (do (merge l a b) o2))
            (ensures eq (merge l a (do (do b o2') o2)) (do (merge l a (do b o2')) o2)) =
   let k = get_key o2' in
   let l' = sel l k in let a' = sel a k in let b' = sel b k in 
-  lemma_merge l a b;
   if get_key o2 = k then
-   one_op_ind_right_s l' a' b' (get_op_s o2) (get_op_s o2')
+   one_op_ind_right_v l' a' b' (get_op_v o2) (get_op_v o2')
   else one_op_ind_right_ne l a b o2 o2'
 
-val one_op_ind_left_s (l a b:concrete_st_s) (o1 o1':op_s) 
+val one_op_ind_left_v (l a b:concrete_st_v) (o1 o1':op_v) 
   : Lemma (requires distinct_ops o1 o1' /\ 
-                    eq_s (merge_s l (do_s a o1) b) (do_s (merge_s l a b) o1))
-           (ensures eq_s (merge_s l (do_s (do_s a o1') o1) b) (do_s (merge_s l (do_s a o1') b) o1))
+                    eq_v (merge_v l (do_v a o1) b) (do_v (merge_v l a b) o1))
+           (ensures eq_v (merge_v l (do_v (do_v a o1') o1) b) (do_v (merge_v l (do_v a o1') b) o1))
 
-val one_op_ind_left_ne (l a b:concrete_st) (o1 o1':op_t)
+let one_op_ind_left_ne (l a b:concrete_st) (o1 o1':op_t)
    : Lemma (requires distinct_ops o1 o1' /\ 
                      ~ (get_key o1 = get_key o1') /\
                     eq (merge l (do a o1) b) (do (merge l a b) o1))
-           (ensures eq (merge l (do (do a o1') o1) b) (do (merge l (do a o1') b) o1))
+           (ensures eq (merge l (do (do a o1') o1) b) (do (merge l (do a o1') b) o1)) = ()
 
 let one_op_ind_left (l a b:concrete_st) (o1 o1':op_t)
    : Lemma (requires distinct_ops o1 o1' /\ eq (merge l (do a o1) b) (do (merge l a b) o1))
            (ensures eq (merge l (do (do a o1') o1) b) (do (merge l (do a o1') b) o1)) =
   let k = get_key o1' in
   let l' = sel l k in let a' = sel a k in let b' = sel b k in 
-  lemma_merge l a b;
   if get_key o1 = k then
-   one_op_ind_left_s l' a' b' (get_op_s o1) (get_op_s o1')
+   one_op_ind_left_v l' a' b' (get_op_v o1) (get_op_v o1')
   else one_op_ind_left_ne l a b o1 o1'
 
-val one_op_ind_lca_s (l:concrete_st_s) (o2 o:op_s) 
+val one_op_ind_lca_v (l:concrete_st_v) (o2 o:op_v) 
   : Lemma (requires distinct_ops o2 o /\ 
-                    eq_s (merge_s l l (do_s l o2)) (do_s l o2))
-          (ensures eq_s (merge_s (do_s l o) (do_s l o) (do_s (do_s l o) o2)) (do_s (do_s l o) o2)) 
+                    eq_v (merge_v l l (do_v l o2)) (do_v l o2))
+          (ensures eq_v (merge_v (do_v l o) (do_v l o) (do_v (do_v l o) o2)) (do_v (do_v l o) o2)) 
 
-val one_op_ind_lca_ne (l:concrete_st) (o2 o:op_t)
+let one_op_ind_lca_ne (l:concrete_st) (o2 o:op_t)
    : Lemma (requires distinct_ops o2 o /\ 
                      ~ (get_key o2 = get_key o) /\
                      eq (merge l l (do l o2)) (do l o2))
-          (ensures eq (merge (do l o) (do l o) (do (do l o) o2)) (do (do l o) o2)) 
+          (ensures eq (merge (do l o) (do l o) (do (do l o) o2)) (do (do l o) o2)) = ()
            
 let one_op_ind_lca (l:concrete_st) (o2 o:op_t)
   : Lemma (requires distinct_ops o2 o /\ eq (merge l l (do l o2)) (do l o2))
@@ -436,19 +446,19 @@ let one_op_ind_lca (l:concrete_st) (o2 o:op_t)
   let k = get_key o in
   let l' = sel l k in 
   if get_key o2 = k then
-   one_op_ind_lca_s l' (get_op_s o2) (get_op_s o)
+   one_op_ind_lca_v l' (get_op_v o2) (get_op_v o)
   else one_op_ind_lca_ne l o2 o
 
 val one_op_base (o2:op_t)
   : Lemma (ensures eq (merge init_st init_st (do init_st o2)) (do init_st o2))
 
-val one_op_inter_base_right_s (l a b c:concrete_st_s) (o2 ob ol:op_s)
-  : Lemma (requires rc_s ob ol <> Either /\ 
+val one_op_inter_base_right_v (l a b c:concrete_st_v) (o2 ob ol:op_v)
+  : Lemma (requires Fst_then_snd? (rc_v ob ol) /\
                     distinct_ops o2 ob /\ distinct_ops o2 ol /\ distinct_ops ob ol /\ 
-                    eq_s (merge_s (do_s l ol) (do_s a ol) (do_s (do_s b ol) o2)) (do_s (do_s c ol) o2) /\
-                    eq_s (merge_s l a (do_s b o2)) (do_s c o2) /\
-                    eq_s (merge_s l (do_s a ol) (do_s b ob)) (do_s (do_s c ob) ol)) //***EXTRA***
-          (ensures eq_s (merge_s (do_s l ol) (do_s a ol) (do_s (do_s (do_s b ob) ol) o2)) (do_s (do_s (do_s c ob) ol) o2))
+                    eq_v (merge_v (do_v l ol) (do_v a ol) (do_v (do_v b ol) o2)) (do_v (do_v c ol) o2) /\
+                    eq_v (merge_v l a (do_v b o2)) (do_v c o2) /\
+                    eq_v (merge_v l (do_v a ol) (do_v b ob)) (do_v (do_v c ob) ol)) //***EXTRA***
+          (ensures eq_v (merge_v (do_v l ol) (do_v a ol) (do_v (do_v (do_v b ob) ol) o2)) (do_v (do_v (do_v c ob) ol) o2))
 
 val one_op_inter_base_right_ne (l a b c:concrete_st) (o2 ob ol:op_t) 
   : Lemma (requires Fst_then_snd? (rc ob ol) /\ 
@@ -469,50 +479,52 @@ let one_op_inter_base_right (l a b c:concrete_st) (o2 ob ol:op_t)
   let k = get_key ob in
   let l' = sel l k in let a' = sel a k in let b' = sel b k in let c' = sel c k in
   if get_key o2 = get_key ob then
-    one_op_inter_base_right_s l' a' b' c' (get_op_s o2) (get_op_s ob) (get_op_s ol)
+    one_op_inter_base_right_v l' a' b' c' (get_op_v o2) (get_op_v ob) (get_op_v ol)
   else one_op_inter_base_right_ne l a b c o2 ob ol
 
-val one_op_inter_base_left_s (l a b c:concrete_st_s) (o2 ob ol:op_s)
-  : Lemma (requires rc_s ob ol <> Either /\ 
+val one_op_inter_base_left_v (l a b c:concrete_st_v) (o2 ob ol:op_v)
+  : Lemma (requires Fst_then_snd? (rc_v ob ol) /\
                     distinct_ops o2 ob /\ distinct_ops o2 ol /\ distinct_ops ob ol /\ 
-                    eq_s (merge_s (do_s l ol) (do_s a ol) (do_s (do_s b ol) o2)) (do_s (do_s c ol) o2) /\
-                    eq_s (merge_s l a (do_s b o2)) (do_s c o2) /\
-                    eq_s (merge_s l (do_s a ol) (do_s b ob)) (do_s (do_s c ob) ol) /\ //***EXTRA***
-                    eq_s (merge_s l (do_s (do_s a ob) ol) (do_s b ol)) (do_s (do_s c ob) ol)) //***EXTRA***
-          (ensures eq_s (merge_s (do_s l ol) (do_s (do_s a ob) ol) (do_s (do_s b ol) o2)) (do_s (do_s (do_s c ob) ol) o2))
+                    eq_v (merge_v (do_v l ol) (do_v a ol) (do_v (do_v b ol) o2)) (do_v (do_v c ol) o2) /\
+                    (Fst_then_snd? (rc_v ob o2) ==> eq_v (merge_v l (do_v a o2) (do_v b ob)) (do_v (merge_v l a (do_v b ob)) o2)) /\ //***EXTRA***
+                    eq_v (merge_v l a (do_v b o2)) (do_v c o2) /\
+                    eq_v (merge_v l (do_v a ob) (do_v b o2)) (do_v (do_v c ob) o2) /\ //EXTRA!! 
+                    eq_v (merge_v l (do_v a ob) (do_v b ol)) (do_v (do_v c ob) ol)) //***EXTRA***
+          (ensures eq_v (merge_v (do_v l ol) (do_v (do_v a ob) ol) (do_v (do_v b ol) o2)) (do_v (do_v (do_v c ob) ol) o2))
 
 val one_op_inter_base_left_ne (l a b c:concrete_st) (o2 ob ol:op_t) 
-  : Lemma (requires Fst_then_snd? (rc ob ol) /\
-                    distinct_ops o2 ob /\ distinct_ops o2 ol /\ distinct_ops ob ol /\
+  : Lemma (requires Fst_then_snd? (rc ob ol) /\ 
+                    distinct_ops ob ol /\ distinct_ops ob o2 /\ distinct_ops ol o2 /\
                     ~ (get_key o2 = get_key ob) /\
                     eq (merge (do l ol) (do a ol) (do (do b ol) o2)) (do (do c ol) o2) /\
                     (Fst_then_snd? (rc ob o2) ==> eq (merge l (do a o2) (do b ob)) (do (merge l a (do b ob)) o2)) /\ //***EXTRA***
                     eq (merge l a (do b o2)) (do c o2) /\
-                    eq (merge l (do a ol) (do b ob)) (do (do c ob) ol) /\ //***EXTRA***
-                    eq (merge l (do (do a ob) ol) (do b ol)) (do (do c ob) ol)) //***EXTRA***
+                    eq (merge l (do a ob) (do b o2)) (do (do c ob) o2) /\ //EXTRA!! 
+                    eq (merge l (do a ob) (do b ol)) (do (do c ob) ol)) //***EXTRA***
           (ensures eq (merge (do l ol) (do (do a ob) ol) (do (do b ol) o2)) (do (do (do c ob) ol) o2))
-          
-let one_op_inter_base_left (l a b c:concrete_st) (o2 ob ol:op_t) 
-  : Lemma (requires Fst_then_snd? (rc ob ol) /\
-                    distinct_ops o2 ob /\ distinct_ops o2 ol /\ distinct_ops ob ol /\
+
+let one_op_inter_base_left (l a b c:concrete_st) (ob ol o2:op_t) 
+  : Lemma (requires Fst_then_snd? (rc ob ol) /\ 
+                    distinct_ops ob ol /\ distinct_ops ob o2 /\ distinct_ops ol o2 /\
                     eq (merge (do l ol) (do a ol) (do (do b ol) o2)) (do (do c ol) o2) /\
                     (Fst_then_snd? (rc ob o2) ==> eq (merge l (do a o2) (do b ob)) (do (merge l a (do b ob)) o2)) /\ //***EXTRA***
                     eq (merge l a (do b o2)) (do c o2) /\
-                    eq (merge l (do a ol) (do b ob)) (do (do c ob) ol) /\ //***EXTRA***
-                    eq (merge l (do (do a ob) ol) (do b ol)) (do (do c ob) ol)) //***EXTRA***
-          (ensures eq (merge (do l ol) (do (do a ob) ol) (do (do b ol) o2)) (do (do (do c ob) ol) o2)) =
+                    eq (merge l (do a ob) (do b o2)) (do (do c ob) o2) /\ //EXTRA!! 
+                    eq (merge l (do a ob) (do b ol)) (do (do c ob) ol)) //***EXTRA***
+          (ensures eq (merge (do l ol) (do (do a ob) ol) (do (do b ol) o2)) (do (do (do c ob) ol) o2)) = 
   let k = get_key ob in
   let l' = sel l k in let a' = sel a k in let b' = sel b k in let c' = sel c k in
   if get_key o2 = get_key ob then
-    one_op_inter_base_left_s l' a' b' c' (get_op_s o2) (get_op_s ob) (get_op_s ol)
+    one_op_inter_base_left_v l' a' b' c' (get_op_v o2) (get_op_v ob) (get_op_v ol)
   else one_op_inter_base_left_ne l a b c o2 ob ol
 
-val one_op_inter_right_s (l a b c:concrete_st_s) (o2 ob ol o:op_s)
-  : Lemma (requires rc_s ob ol <> Either /\ 
+val one_op_inter_right_v (l a b c:concrete_st_v) (o2 ob ol o:op_v)
+  : Lemma (requires Fst_then_snd? (rc_v ob ol) /\
                     distinct_ops o ob /\ distinct_ops o ol /\ distinct_ops o o2 /\ distinct_ops ob ol /\ distinct_ops ob o2 /\ distinct_ops o2 ol /\
                     get_rid o <> get_rid ol /\
-                    eq_s (merge_s (do_s l ol) (do_s a ol) (do_s (do_s (do_s b ob) ol) o2)) (do_s (do_s (do_s c ob) ol) o2))
-      (ensures eq_s (merge_s (do_s l ol) (do_s a ol) (do_s (do_s (do_s (do_s b o) ob) ol) o2)) (do_s (do_s (do_s (do_s c o) ob) ol) o2))
+                    ((~ (commutes_with_v o ob)) \/ Fst_then_snd? (rc_v o ol)) /\
+                    eq_v (merge_v (do_v l ol) (do_v a ol) (do_v (do_v (do_v b ob) ol) o2)) (do_v (do_v (do_v c ob) ol) o2))
+      (ensures eq_v (merge_v (do_v l ol) (do_v a ol) (do_v (do_v (do_v (do_v b o) ob) ol) o2)) (do_v (do_v (do_v (do_v c o) ob) ol) o2))
 
 val one_op_inter_right_ne (l a b c:concrete_st) (o2 ob ol o:op_t) 
   : Lemma (requires Fst_then_snd? (rc ob ol) /\
@@ -533,15 +545,16 @@ let one_op_inter_right (l a b c:concrete_st) (o2 ob ol o:op_t)
   let k = get_key o in
   let l' = sel l k in let a' = sel a k in let b' = sel b k in let c' = sel c k in
   if get_key o2 = get_key ob then 
-    one_op_inter_right_s l' a' b' c' (get_op_s o2) (get_op_s ob) (get_op_s ol) (get_op_s o)
+    one_op_inter_right_v l' a' b' c' (get_op_v o2) (get_op_v ob) (get_op_v ol) (get_op_v o)
   else one_op_inter_right_ne l a b c o2 ob ol o
 
-val one_op_inter_left_s (l a b c:concrete_st_s) (o2 ob ol o:op_s)
-  : Lemma (requires rc_s ob ol <> Either /\ 
+val one_op_inter_left_v (l a b c:concrete_st_v) (o2 ob ol o:op_v)
+  : Lemma (requires Fst_then_snd? (rc_v ob ol) /\
                     distinct_ops o ob /\ distinct_ops o ol /\ distinct_ops o o2 /\ distinct_ops ob ol /\ distinct_ops ob o2 /\ distinct_ops o2 ol /\
                     get_rid o <> get_rid ol /\
-                    eq_s (merge_s (do_s l ol) (do_s (do_s a ob) ol) (do_s (do_s b ol) o2)) (do_s (do_s (do_s c ob) ol) o2))
-          (ensures eq_s (merge_s (do_s l ol) (do_s (do_s (do_s a o) ob) ol) (do_s (do_s b ol) o2)) (do_s (do_s (do_s (do_s c o) ob) ol) o2))
+                    ((~ (commutes_with_v o ob)) \/ Fst_then_snd? (rc_v o ol)) /\
+                    eq_v (merge_v (do_v l ol) (do_v (do_v a ob) ol) (do_v (do_v b ol) o2)) (do_v (do_v (do_v c ob) ol) o2))
+          (ensures eq_v (merge_v (do_v l ol) (do_v (do_v (do_v a o) ob) ol) (do_v (do_v b ol) o2)) (do_v (do_v (do_v (do_v c o) ob) ol) o2))
 
 val one_op_inter_left_ne (l a b c:concrete_st) (o2 ob ol o:op_t) 
   : Lemma (requires Fst_then_snd? (rc ob ol) /\
@@ -562,16 +575,16 @@ let one_op_inter_left (l a b c:concrete_st) (o2 ob ol o:op_t)
   let k = get_key o in
   let l' = sel l k in let a' = sel a k in let b' = sel b k in let c' = sel c k in
   if get_key o2 = get_key ob then 
-    one_op_inter_left_s l' a' b' c' (get_op_s o2) (get_op_s ob) (get_op_s ol) (get_op_s o)
+    one_op_inter_left_v l' a' b' c' (get_op_v o2) (get_op_v ob) (get_op_v ol) (get_op_v o)
   else one_op_inter_left_ne l a b c o2 ob ol o
 
-val one_op_inter_lca_s (l a b c:concrete_st_s) (o2 ol oi:op_s)
+val one_op_inter_lca_v (l a b c:concrete_st_v) (o2 ol oi:op_v)
   : Lemma (requires distinct_ops o2 ol /\ distinct_ops o2 oi /\ distinct_ops ol oi /\ 
-                    (exists o. rc_s o ol <> Either) /\ 
-                    (exists o. rc_s o oi <> Either) /\
-                    eq_s (merge_s (do_s l oi) (do_s a oi) (do_s (do_s b oi) o2)) (do_s (do_s c oi) o2) /\
-                    eq_s (merge_s (do_s l ol) (do_s a ol) (do_s (do_s b ol) o2)) (do_s (do_s c ol) o2))
-    (ensures eq_s (merge_s (do_s (do_s l oi) ol) (do_s (do_s a oi) ol) (do_s (do_s (do_s b oi) ol) o2)) (do_s (do_s (do_s c oi) ol) o2))
+                    (exists o. Fst_then_snd? (rc_v o ol)) /\ 
+                    (exists o. Fst_then_snd? (rc_v o oi)) /\
+                    eq_v (merge_v (do_v l oi) (do_v a oi) (do_v (do_v b oi) o2)) (do_v (do_v c oi) o2) /\
+                    eq_v (merge_v (do_v l ol) (do_v a ol) (do_v (do_v b ol) o2)) (do_v (do_v c ol) o2))
+    (ensures eq_v (merge_v (do_v (do_v l oi) ol) (do_v (do_v a oi) ol) (do_v (do_v (do_v b oi) ol) o2)) (do_v (do_v (do_v c oi) ol) o2))
 
 val one_op_inter_lca_ne (l a b c:concrete_st) (o2 ol oi:op_t)
   : Lemma (requires distinct_ops o2 ol /\ distinct_ops o2 oi /\ distinct_ops ol oi /\ 
@@ -593,17 +606,18 @@ let one_op_inter_lca (l a b c:concrete_st) (o2 ol oi:op_t)
   let k = get_key oi in
   let l' = sel l k in let a' = sel a k in let b' = sel b k in let c' = sel c k in
   if get_key o2 = k && get_key o2 = get_key ol then 
-    one_op_inter_lca_s l' a' b' c' (get_op_s o2) (get_op_s ol) (get_op_s oi)
+    one_op_inter_lca_v l' a' b' c' (get_op_v o2) (get_op_v ol) (get_op_v oi)
   else one_op_inter_lca_ne l a b c o2 ol oi
 
 (*Zero op *)
 ///////////////
-val zero_op_inter_base_right_s (l a b c:concrete_st_s) (ob ol:op_s)
-  : Lemma (requires rc_s ob ol <> Either /\ distinct_ops ob ol /\ 
-                    eq_s (merge_s (do_s l ol) (do_s a ol) (do_s b ol)) (do_s c ol) /\
-                    eq_s (merge_s l a b) c /\
-                    eq_s (merge_s l (do_s a ol) (do_s b ob)) (do_s (do_s c ob) ol)) //***EXTRA***
-          (ensures eq_s (merge_s (do_s l ol) (do_s a ol) (do_s (do_s b ob) ol)) (do_s (do_s c ob) ol))
+val zero_op_inter_base_right_v (l a b c:concrete_st_v) (ob ol:op_v)
+  : Lemma (requires Fst_then_snd? (rc_v ob ol) /\ 
+                    distinct_ops ob ol /\ 
+                    eq_v (merge_v (do_v l ol) (do_v a ol) (do_v b ol)) (do_v c ol) /\
+                    eq_v (merge_v l a b) c /\
+                    eq_v (merge_v l (do_v a ol) (do_v b ob)) (do_v (do_v c ob) ol)) //***EXTRA***
+          (ensures eq_v (merge_v (do_v l ol) (do_v a ol) (do_v (do_v b ob) ol)) (do_v (do_v c ob) ol))
 
 // because we proved that e_i^l rcp eb is not possible.
 //e_i^l vis eb is not possible
@@ -616,15 +630,15 @@ let zero_op_inter_base_right (l a b c:concrete_st) (ob ol:op_t)
           (ensures eq (merge (do l ol) (do a ol) (do (do b ob) ol)) (do (do c ob) ol)) =
   let k = get_key ob in
   let l' = sel l k in let a' = sel a k in let b' = sel b k in let c' = sel c k in
-  lemma_merge l a b;
-  zero_op_inter_base_right_s l' a' b' c' (get_op_s ob) (get_op_s ol)
+  zero_op_inter_base_right_v l' a' b' c' (get_op_v ob) (get_op_v ol)
 
-val zero_op_inter_base_left_s (l a b c:concrete_st_s) (ob ol:op_s)
-  : Lemma (requires rc_s ob ol <> Either /\ distinct_ops ob ol /\ 
-                    eq_s (merge_s (do_s l ol) (do_s a ol) (do_s b ol)) (do_s c ol) /\
-                    eq_s (merge_s l a b) c /\
-                    eq_s (merge_s l (do_s a ob) (do_s b ol)) (do_s (do_s c ob) ol)) //***EXTRA***
-          (ensures eq_s (merge_s (do_s l ol) (do_s (do_s a ob) ol) (do_s b ol)) (do_s (do_s c ob) ol))
+val zero_op_inter_base_left_v (l a b c:concrete_st_v) (ob ol:op_v)
+  : Lemma (requires Fst_then_snd? (rc_v ob ol) /\ 
+                    distinct_ops ob ol /\ 
+                    eq_v (merge_v (do_v l ol) (do_v a ol) (do_v b ol)) (do_v c ol) /\
+                    eq_v (merge_v l a b) c /\
+                    eq_v (merge_v l (do_v a ob) (do_v b ol)) (do_v (do_v c ob) ol)) //***EXTRA***
+          (ensures eq_v (merge_v (do_v l ol) (do_v (do_v a ob) ol) (do_v b ol)) (do_v (do_v c ob) ol))
           
 let zero_op_inter_base_left (l a b c:concrete_st) (ob ol:op_t) 
   : Lemma (requires Fst_then_snd? (rc ob ol) /\ distinct_ops ob ol /\ 
@@ -634,14 +648,15 @@ let zero_op_inter_base_left (l a b c:concrete_st) (ob ol:op_t)
           (ensures eq (merge (do l ol) (do (do a ob) ol) (do b ol) ) (do (do c ob) ol)) =
   let k = get_key ob in
   let l' = sel l k in let a' = sel a k in let b' = sel b k in let c' = sel c k in
-  lemma_merge l a b;
-  zero_op_inter_base_left_s l' a' b' c' (get_op_s ob) (get_op_s ol)
+  zero_op_inter_base_left_v l' a' b' c' (get_op_v ob) (get_op_v ol)
 
-val zero_op_inter_right_s (l a b c:concrete_st_s) (ob ol o:op_s)
-  : Lemma (requires rc_s ob ol <> Either /\ distinct_ops ob ol /\ distinct_ops ob o /\ distinct_ops ol o /\
+val zero_op_inter_right_v (l a b c:concrete_st_v) (ob ol o:op_v)
+  : Lemma (requires Fst_then_snd? (rc_v ob ol) /\ 
+                    distinct_ops ob ol /\ distinct_ops ob o /\ distinct_ops ol o /\
                     get_rid o <> get_rid ol (*o,ol must be concurrent*) /\
-                    eq_s (merge_s (do_s l ol) (do_s a ol) (do_s (do_s b ob) ol)) (do_s (do_s c ob) ol))
-          (ensures eq_s (merge_s (do_s l ol) (do_s a ol) (do_s (do_s (do_s b o) ob) ol)) (do_s (do_s (do_s c o) ob) ol)) 
+                    ((~ (commutes_with_v o ob)) \/ Fst_then_snd? (rc_v o ol)) /\
+                    eq_v (merge_v (do_v l ol) (do_v a ol) (do_v (do_v b ob) ol)) (do_v (do_v c ob) ol))
+          (ensures eq_v (merge_v (do_v l ol) (do_v a ol) (do_v (do_v (do_v b o) ob) ol)) (do_v (do_v (do_v c o) ob) ol)) 
           
 let zero_op_inter_right (l a b c:concrete_st) (ob ol o:op_t)
   : Lemma (requires Fst_then_snd? (rc ob ol) /\ 
@@ -652,13 +667,15 @@ let zero_op_inter_right (l a b c:concrete_st) (ob ol o:op_t)
           (ensures eq (merge (do l ol) (do a ol) (do (do (do b o) ob) ol)) (do (do (do c o) ob) ol)) =
   let k = get_key ob in
   let l' = sel l k in let a' = sel a k in let b' = sel b k in let c' = sel c k in
-  zero_op_inter_right_s l' a' b' c' (get_op_s ob) (get_op_s ol) (get_op_s o)
+  zero_op_inter_right_v l' a' b' c' (get_op_v ob) (get_op_v ol) (get_op_v o)
 
-val zero_op_inter_left_s (l a b c:concrete_st_s) (ob ol o:op_s)
-  : Lemma (requires rc_s ob ol <> Either /\ distinct_ops ob ol /\ distinct_ops ob o /\ distinct_ops ol o /\
+val zero_op_inter_left_v (l a b c:concrete_st_v) (ob ol o:op_v)
+  : Lemma (requires Fst_then_snd? (rc_v ob ol) /\
+                    distinct_ops ob ol /\ distinct_ops ob o /\ distinct_ops ol o /\
                     get_rid o <> get_rid ol (*o,ol must be concurrent*) /\
-                    eq_s (merge_s (do_s l ol) (do_s (do_s a ob) ol) (do_s b ol)) (do_s (do_s c ob) ol))
-          (ensures eq_s (merge_s (do_s l ol) (do_s (do_s (do_s a o) ob) ol) (do_s b ol)) (do_s (do_s (do_s c o) ob) ol)) 
+                    ((~ (commutes_with_v o ob)) \/ Fst_then_snd? (rc_v o ol)) /\
+                    eq_v (merge_v (do_v l ol) (do_v (do_v a ob) ol) (do_v b ol)) (do_v (do_v c ob) ol))
+          (ensures eq_v (merge_v (do_v l ol) (do_v (do_v (do_v a o) ob) ol) (do_v b ol)) (do_v (do_v (do_v c o) ob) ol)) 
           
 let zero_op_inter_left (l a b c:concrete_st) (ob ol o:op_t)
   : Lemma (requires Fst_then_snd? (rc ob ol) /\ 
@@ -669,11 +686,11 @@ let zero_op_inter_left (l a b c:concrete_st) (ob ol o:op_t)
           (ensures eq (merge (do l ol) (do (do (do a o) ob) ol) (do b ol)) (do (do (do c o) ob) ol)) =
   let k = get_key ob in
   let l' = sel l k in let a' = sel a k in let b' = sel b k in let c' = sel c k in
-  zero_op_inter_left_s l' a' b' c' (get_op_s ob) (get_op_s ol) (get_op_s o)
+  zero_op_inter_left_v l' a' b' c' (get_op_v ob) (get_op_v ol) (get_op_v o)
 
-val zero_op_inter_lca_v1_s (l a b c:concrete_st_s) (ol:op_s)
-  : Lemma (requires (exists o'. rc_s o' ol <> Either) /\ eq_s (merge_s l a b) c)
-          (ensures eq_s (merge_s (do_s l ol) (do_s a ol) (do_s b ol)) (do_s c ol))
+val zero_op_inter_lca_v1_v (l a b c:concrete_st_v) (ol:op_v)
+  : Lemma (requires (exists o'. Fst_then_snd? (rc_v o' ol)) /\ eq_v (merge_v l a b) c)
+          (ensures eq_v (merge_v (do_v l ol) (do_v a ol) (do_v b ol)) (do_v c ol))
 
 // In general, the event "o" below should be such that these exists o', (rc o' o)
 let zero_op_inter_lca_v1 (l a b c:concrete_st) (ol:op_t)
@@ -681,16 +698,15 @@ let zero_op_inter_lca_v1 (l a b c:concrete_st) (ol:op_t)
           (ensures eq (merge (do l ol) (do a ol) (do b ol)) (do c ol)) =
   let k = get_key ol in
   let l' = sel l k in let a' = sel a k in let b' = sel b k in let c' = sel c k in
-  lemma_merge l a b;
-  zero_op_inter_lca_v1_s l' a' b' c' (get_op_s ol)
+  zero_op_inter_lca_v1_v l' a' b' c' (get_op_v ol)
 
-val zero_op_inter_lca_v2_s (l a b c:concrete_st_s) (ol oi:op_s)
+val zero_op_inter_lca_v2_v (l a b c:concrete_st_v) (ol oi:op_v)
   : Lemma (requires distinct_ops ol oi /\
-                    (exists o. rc_s o ol <> Either) /\ 
-                    (exists o. rc_s o oi <> Either) /\ 
-                    eq_s (merge_s (do_s l oi) (do_s a oi) (do_s b oi)) (do_s c oi)  /\
-                    eq_s (merge_s (do_s l ol) (do_s a ol) (do_s b ol)) (do_s c ol))
-          (ensures eq_s (merge_s (do_s (do_s l oi) ol) (do_s (do_s a oi) ol) (do_s (do_s b oi) ol)) (do_s (do_s c oi) ol))
+                    (exists o. Fst_then_snd? (rc_v o ol)) /\ 
+                    (exists o. Fst_then_snd? (rc_v o oi)) /\ 
+                    eq_v (merge_v (do_v l oi) (do_v a oi) (do_v b oi)) (do_v c oi)  /\
+                    eq_v (merge_v (do_v l ol) (do_v a ol) (do_v b ol)) (do_v c ol))
+          (ensures eq_v (merge_v (do_v (do_v l oi) ol) (do_v (do_v a oi) ol) (do_v (do_v b oi) ol)) (do_v (do_v c oi) ol))
 
 val zero_op_inter_lca_v2_ne (l a b c:concrete_st) (ol oi:op_t)
   : Lemma (requires distinct_ops ol oi /\
@@ -712,60 +728,86 @@ let zero_op_inter_lca_v2 (l a b c:concrete_st) (ol oi:op_t)
   let k = get_key ol in
   let l' = sel l k in let a' = sel a k in let b' = sel b k in let c' = sel c k in
   if get_key oi = k then
-    zero_op_inter_lca_v2_s l' a' b' c' (get_op_s ol) (get_op_s oi)
+    zero_op_inter_lca_v2_v l' a' b' c' (get_op_v ol) (get_op_v oi)
   else zero_op_inter_lca_v2_ne l a b c ol oi
           
 (*Two OP COMM*)
 //////////////// 
 
-//simpler MRDT lemma (Already proved for Grows-only set)
-val comm_ind_right_s (l a b:concrete_st_s) (o1 o2' o2:op_s)
-  : Lemma (requires eq_s (merge_s l (do_s a o1) (do_s b o2)) (do_s (do_s (merge_s l a b) o2) o1))
-          (ensures eq_s (merge_s l (do_s a o1) (do_s (do_s b o2') o2)) (do_s (do_s (merge_s l a (do_s b o2')) o2) o1))
+val comm_ind_right_v (l a b:concrete_st_v) (o1 o2' o2:op_v)
+  : Lemma (requires Either? (rc_v o1 o2) /\
+                    (Fst_then_snd? (rc_v o2' o1) ==> (eq_v (merge_v l (do_v a o1) (do_v b o2')) (do_v (merge_v l a (do_v b o2')) o1))) /\
+                    ~ (Fst_then_snd? (rc_v o1 o2')) /\
+                    eq_v (merge_v l (do_v a o1) (do_v b o2)) (do_v (do_v (merge_v l a b) o2) o1))
+          (ensures eq_v (merge_v l (do_v a o1) (do_v (do_v b o2') o2)) (do_v (do_v (merge_v l a (do_v b o2')) o2) o1))
 
 val comm_ind_right_ne (l a b:concrete_st) (o1 o2' o2:op_t)
-  : Lemma (requires Either? (rc o1 o2) /\
-                     ~ (get_key o1 = get_key o2 /\ get_key o2 = get_key o2') /\
-                    eq (merge l (do a o1) (do b o2)) (do (do (merge l a b) o2) o1))                    
+  : Lemma (requires Either? (rc o1 o2) /\ 
+                    distinct_ops o1 o2 /\ distinct_ops o1 o2' /\ distinct_ops o2 o2' /\
+                    ~ (get_key o1 = get_key o2 /\ get_key o2 = get_key o2') /\
+                    eq (merge l (do a o1) (do b o2)) (do (do (merge l a b) o2) o1) /\
+                    (Fst_then_snd? (rc o2' o1) ==> (eq (merge l (do a o1) (do b o2')) (do (merge l a (do b o2')) o1))) /\
+                    ~ (exists o3 a'. eq (do a o1) (do a' o3) /\ distinct_ops o2 o3 /\ Fst_then_snd? (rc o2 o3)) /\
+                    ~ (Fst_then_snd? (rc o1 o2')) /\
+                    ~ (exists o3 b'. eq (do (do b o2') o2) (do b' o3) /\ distinct_ops o1 o3 /\ Fst_then_snd? (rc o1 o3)) /\
+                    ~ (exists o3 b'. eq (do b o2) (do b' o3) /\ distinct_ops o1 o3 /\ Fst_then_snd? (rc o1 o3)))                    
           (ensures eq (merge l (do a o1) (do (do b o2') o2)) (do (do (merge l a (do b o2')) o2) o1)) 
           
 let comm_ind_right (l a b:concrete_st) (o1 o2' o2:op_t)
   : Lemma (requires Either? (rc o1 o2) /\ 
-                    eq (merge l (do a o1) (do b o2)) (do (do (merge l a b) o2) o1))                    
+                    distinct_ops o1 o2 /\ distinct_ops o1 o2' /\ distinct_ops o2 o2' /\
+                    eq (merge l (do a o1) (do b o2)) (do (do (merge l a b) o2) o1) /\
+                    (Fst_then_snd? (rc o2' o1) ==> (eq (merge l (do a o1) (do b o2')) (do (merge l a (do b o2')) o1))) /\
+                    ~ (exists o3 a'. eq (do a o1) (do a' o3) /\ distinct_ops o2 o3 /\ Fst_then_snd? (rc o2 o3)) /\
+                    ~ (Fst_then_snd? (rc o1 o2')) /\
+                    ~ (exists o3 b'. eq (do (do b o2') o2) (do b' o3) /\ distinct_ops o1 o3 /\ Fst_then_snd? (rc o1 o3)) /\
+                    ~ (exists o3 b'. eq (do b o2) (do b' o3) /\ distinct_ops o1 o3 /\ Fst_then_snd? (rc o1 o3)))                    
           (ensures eq (merge l (do a o1) (do (do b o2') o2)) (do (do (merge l a (do b o2')) o2) o1)) =
   let k = get_key o2' in
   let l' = sel l k in let a' = sel a k in let b' = sel b k in 
-  lemma_merge l a b;
-  if get_key o2 = get_key o1 && get_key o1 = k then 
-    comm_ind_right_s l' a' b' (get_op_s o1) (get_op_s o2') (get_op_s o2)
+  if get_key o2 = get_key o1 && get_key o1 = k && Either? (rc_v (get_op_v o1) (get_op_v o2)) then 
+    comm_ind_right_v l' a' b' (get_op_v o1) (get_op_v o2') (get_op_v o2)
   else comm_ind_right_ne l a b o1 o2' o2
 
-//simpler MRDT lemma (Already proved for Grows-only set)
-val comm_ind_left_s (l a b:concrete_st_s) (o1 o2' o2:op_s)
-  : Lemma (requires eq_s (merge_s l (do_s a o1) (do_s b o2)) (do_s (do_s (merge_s l a b) o2) o1))
-          (ensures eq_s (merge_s l (do_s (do_s a o2') o1) (do_s b o2)) (do_s (do_s (merge_s l (do_s a o2') b) o2) o1))
+val comm_ind_left_v (l a b:concrete_st_v) (o1 o2 o1':op_v)
+  : Lemma (requires Either? (rc_v o1 o2) /\
+                    (Fst_then_snd? (rc_v o1' o2) ==> (eq_v (merge_v l (do_v a o1') (do_v b o2)) (do_v (merge_v l (do_v a o1') b) o2))) /\
+                    ~ (Fst_then_snd? (rc_v o2 o1')) /\
+                    eq_v (merge_v l (do_v a o1) (do_v b o2)) (do_v (do_v (merge_v l a b) o2) o1))
+          (ensures eq_v (merge_v l (do_v (do_v a o1') o1) (do_v b o2)) (do_v (do_v (merge_v l (do_v a o1') b) o2) o1))
 
-val comm_ind_left_ne (l a b:concrete_st) (o1 o2' o2:op_t)
+val comm_ind_left_ne (l a b:concrete_st) (o1 o2 o1':op_t)
   : Lemma (requires Either? (rc o1 o2) /\ 
-                    ~ (get_key o1 = get_key o2 /\ get_key o2 = get_key o2') /\
-                    eq (merge l (do a o1) (do b o2)) (do (do (merge l a b) o2) o1))                    
-          (ensures eq (merge l (do (do a o2') o1) (do b o2)) (do (do (merge l (do a o2') b) o2) o1)) 
+                    distinct_ops o1 o2 /\ distinct_ops o1 o1' /\ distinct_ops o2 o1' /\
+                    ~ (get_key o1 = get_key o2 /\ get_key o2 = get_key o1') /\
+                    eq (merge l (do a o1) (do b o2)) (do (do (merge l a b) o2) o1) /\
+                    (Fst_then_snd? (rc o1' o2) ==> (eq (merge l (do a o1') (do b o2)) (do (merge l (do a o1') b) o2))) /\
+                    ~ (exists o3 a'. eq (do a o1) (do a' o3) /\ distinct_ops o2 o3 /\ Fst_then_snd? (rc o2 o3)) /\
+                    ~ (Fst_then_snd? (rc o2 o1')) /\
+                    ~ (exists o3 b'. eq (do (do b o1') o2) (do b' o3) /\ distinct_ops o1 o3 /\ Fst_then_snd? (rc o1 o3)) /\
+                    ~ (exists o3 b'. eq (do b o2) (do b' o3) /\ distinct_ops o1 o3 /\ Fst_then_snd? (rc o1 o3)))                    
+          (ensures eq (merge l (do (do a o1') o1) (do b o2)) (do (do (merge l (do a o1') b) o2) o1))
           
-let comm_ind_left (l a b:concrete_st) (o1 o2' o2:op_t)
+let comm_ind_left (l a b:concrete_st) (o1 o2 o1':op_t)
   : Lemma (requires Either? (rc o1 o2) /\ 
-                    eq (merge l (do a o1) (do b o2)) (do (do (merge l a b) o2) o1))                    
-          (ensures eq (merge l (do (do a o2') o1) (do b o2)) (do (do (merge l (do a o2') b) o2) o1)) =
-  let k = get_key o2' in
+                    distinct_ops o1 o2 /\ distinct_ops o1 o1' /\ distinct_ops o2 o1' /\
+                    eq (merge l (do a o1) (do b o2)) (do (do (merge l a b) o2) o1) /\
+                    (Fst_then_snd? (rc o1' o2) ==> (eq (merge l (do a o1') (do b o2)) (do (merge l (do a o1') b) o2))) /\
+                    ~ (exists o3 a'. eq (do a o1) (do a' o3) /\ distinct_ops o2 o3 /\ Fst_then_snd? (rc o2 o3)) /\
+                    ~ (Fst_then_snd? (rc o2 o1')) /\
+                    ~ (exists o3 b'. eq (do (do b o1') o2) (do b' o3) /\ distinct_ops o1 o3 /\ Fst_then_snd? (rc o1 o3)) /\
+                    ~ (exists o3 b'. eq (do b o2) (do b' o3) /\ distinct_ops o1 o3 /\ Fst_then_snd? (rc o1 o3)))                    
+          (ensures eq (merge l (do (do a o1') o1) (do b o2)) (do (do (merge l (do a o1') b) o2) o1)) =
+  let k = get_key o1' in
   let l' = sel l k in let a' = sel a k in let b' = sel b k in 
-  lemma_merge l a b;
   if get_key o2 = get_key o1 && get_key o1 = k then 
-    comm_ind_left_s l' a' b' (get_op_s o1) (get_op_s o2') (get_op_s o2)
-  else comm_ind_left_ne l a b o1 o2' o2
+    comm_ind_left_v l' a' b' (get_op_v o1) (get_op_v o2) (get_op_v o1')
+  else comm_ind_left_ne l a b o1 o2 o1'
 
-//simpler MRDT lemma (Already proved for Grows-only set)
-val comm_ind_lca_s (l:concrete_st_s) (ol o1 o2:op_s)
-  : Lemma (requires eq_s (merge_s l (do_s l o1) (do_s l o2)) (do_s (do_s l o2) o1))
-          (ensures eq_s (merge_s (do_s l ol) (do_s (do_s l ol) o1) (do_s (do_s l ol) o2)) (do_s (do_s (do_s l ol) o2) o1))
+val comm_ind_lca_v (l:concrete_st_v) (ol o1 o2:op_v)
+  : Lemma (requires Either? (rc_v o1 o2) /\
+                    eq_v (merge_v l (do_v l o1) (do_v l o2)) (do_v (do_v l o2) o1))
+          (ensures eq_v (merge_v (do_v l ol) (do_v (do_v l ol) o1) (do_v (do_v l ol) o2)) (do_v (do_v (do_v l ol) o2) o1))
 
 val comm_ind_lca_ne (l:concrete_st) (ol o1 o2:op_t)
   : Lemma (requires Either? (rc o1 o2) /\ 
@@ -780,24 +822,24 @@ let comm_ind_lca (l:concrete_st) (ol o1 o2:op_t)
   let k = get_key ol in
   let l' = sel l k in
   if get_key ol = get_key o1 && get_key ol = get_key o2 then
-    comm_ind_lca_s l' (get_op_s ol) (get_op_s o1) (get_op_s o2)
+    comm_ind_lca_v l' (get_op_v ol) (get_op_v o1) (get_op_v o2)
   else comm_ind_lca_ne l ol o1 o2
 
 val comm_base (o1 o2:op_t)
   : Lemma (requires Either? (rc o1 o2) /\ distinct_ops o1 o2)
           (ensures eq (merge init_st (do init_st o1) (do init_st o2)) (do (do init_st o1) o2))
 
-val comm_inter_base_right_s (l a b c:concrete_st_s) (o1 o2 ob ol:op_s) 
-  : Lemma (requires rc_s ob ol <> Either /\ 
+val comm_inter_base_right_v (l a b c:concrete_st_v) (o1 o2 ob ol:op_v) 
+  : Lemma (requires Either? (rc_v o1 o2) /\ Fst_then_snd? (rc_v ob ol) /\ 
                     distinct_ops o1 o2 /\ distinct_ops o1 ob /\ distinct_ops o1 ol /\ distinct_ops o2 ob /\ distinct_ops o2 ol /\ distinct_ops ob ol /\
-                    eq_s (merge_s (do_s l ol) (do_s (do_s a ol) o1) (do_s (do_s b ol) o2)) (do_s (do_s (do_s c ol) o1) o2) /\ 
-                    eq_s (merge_s l (do_s a o1) (do_s b o2)) (do_s (do_s c o1) o2) /\
-                    eq_s (merge_s l (do_s a o1) (do_s (do_s b ob) o2)) (do_s (do_s (merge_s l a (do_s b ob)) o1) o2) /\ //comes from comm_ind_right
-                    eq_s (merge_s (do_s l ol) (do_s a ol) (do_s (do_s b ob) ol)) (do_s (do_s c ob) ol)) //comes from intermediate_base_zero_op
-          (ensures eq_s (merge_s (do_s l ol) (do_s (do_s a ol) o1) (do_s (do_s (do_s b ob) ol) o2)) (do_s (do_s (do_s (do_s c ob) ol) o1) o2))
+                    eq_v (merge_v (do_v l ol) (do_v (do_v a ol) o1) (do_v (do_v b ol) o2)) (do_v (do_v (do_v c ol) o1) o2) /\ 
+                    eq_v (merge_v l (do_v a o1) (do_v b o2)) (do_v (do_v c o1) o2) /\
+                    eq_v (merge_v l (do_v a o1) (do_v (do_v b ob) o2)) (do_v (do_v (merge_v l a (do_v b ob)) o1) o2) /\ //comes from comm_ind_right
+                    eq_v (merge_v (do_v l ol) (do_v a ol) (do_v (do_v b ob) ol)) (do_v (do_v c ob) ol)) //comes from intermediate_base_zero_op
+          (ensures eq_v (merge_v (do_v l ol) (do_v (do_v a ol) o1) (do_v (do_v (do_v b ob) ol) o2)) (do_v (do_v (do_v (do_v c ob) ol) o1) o2))
 
 val comm_inter_base_right_ne (l a b c:concrete_st) (o1 o2 ob ol:op_t) 
-  : Lemma (requires Fst_then_snd? (rc ob ol) /\ 
+  : Lemma (requires Either? (rc o1 o2) /\ Fst_then_snd? (rc ob ol) /\ 
                     distinct_ops o1 o2 /\ distinct_ops o1 ob /\ distinct_ops o1 ol /\ distinct_ops o2 ob /\ distinct_ops o2 ol /\ distinct_ops ob ol /\
                     ~ (get_key o2 = get_key o1 /\ get_key o1 = get_key ob) /\
                     eq (merge (do l ol) (do (do a ol) o1) (do (do b ol) o2)) (do (do (do c ol) o1) o2) /\ 
@@ -817,20 +859,20 @@ let comm_inter_base_right (l a b c:concrete_st) (o1 o2 ob ol:op_t)
   let k = get_key ob in
   let l' = sel l k in let a' = sel a k in let b' = sel b k in let c' = sel c k in
   if get_key o2 = get_key o1 && get_key o1 = k then 
-    comm_inter_base_right_s l' a' b' c' (get_op_s o1) (get_op_s o2) (get_op_s ob) (get_op_s ol)
+    comm_inter_base_right_v l' a' b' c' (get_op_v o1) (get_op_v o2) (get_op_v ob) (get_op_v ol)
   else comm_inter_base_right_ne l a b c o1 o2 ob ol
 
-val comm_inter_base_left_s (l a b c:concrete_st_s) (o1 o2 ob ol:op_s) 
-  : Lemma (requires rc_s ob ol <> Either /\ 
+val comm_inter_base_left_v (l a b c:concrete_st_v) (o1 o2 ob ol:op_v) 
+  : Lemma (requires Either? (rc_v o1 o2) /\ Fst_then_snd? (rc_v ob ol) /\ 
                     distinct_ops o1 o2 /\ distinct_ops o1 ob /\ distinct_ops o1 ol /\ distinct_ops o2 ob /\ distinct_ops o2 ol /\ distinct_ops ob ol /\
-                    eq_s (merge_s (do_s l ol) (do_s (do_s a ol) o1) (do_s (do_s b ol) o2)) (do_s (do_s (do_s c ol) o1) o2) /\ 
-                    eq_s (merge_s l (do_s a o1) (do_s b o2)) (do_s (do_s c o1) o2) /\
-                    eq_s (merge_s l (do_s (do_s a ob) o1) (do_s b o2)) (do_s (do_s (merge_s l (do_s a ob) b) o1) o2) /\ //comes from comm_ind_left
-                    eq_s (merge_s (do_s l ol) (do_s (do_s a ob) ol) (do_s b ol)) (do_s (do_s c ob) ol)) //comes from intermediate_base_zero_op
-          (ensures eq_s (merge_s (do_s l ol) (do_s (do_s (do_s a ob) ol) o1) (do_s (do_s b ol) o2)) (do_s (do_s (do_s (do_s c ob) ol) o1) o2))
+                    eq_v (merge_v (do_v l ol) (do_v (do_v a ol) o1) (do_v (do_v b ol) o2)) (do_v (do_v (do_v c ol) o1) o2) /\ 
+                    eq_v (merge_v l (do_v a o1) (do_v b o2)) (do_v (do_v c o1) o2) /\
+                    eq_v (merge_v l (do_v (do_v a ob) o1) (do_v b o2)) (do_v (do_v (merge_v l (do_v a ob) b) o1) o2) /\ //comes from comm_ind_left
+                    eq_v (merge_v (do_v l ol) (do_v (do_v a ob) ol) (do_v b ol)) (do_v (do_v c ob) ol)) //comes from intermediate_base_zero_op
+          (ensures eq_v (merge_v (do_v l ol) (do_v (do_v (do_v a ob) ol) o1) (do_v (do_v b ol) o2)) (do_v (do_v (do_v (do_v c ob) ol) o1) o2))
 
 val comm_inter_base_left_ne (l a b c:concrete_st) (o1 o2 ob ol:op_t) 
-  : Lemma (requires Fst_then_snd? (rc ob ol) /\ 
+  : Lemma (requires Either? (rc o1 o2) /\ Fst_then_snd? (rc ob ol) /\ 
                     distinct_ops o1 o2 /\ distinct_ops o1 ob /\ distinct_ops o1 ol /\ distinct_ops o2 ob /\ distinct_ops o2 ol /\ distinct_ops ob ol /\
                     ~ (get_key o2 = get_key o1 /\ get_key o1 = get_key ob) /\
                     eq (merge (do l ol) (do (do a ol) o1) (do (do b ol) o2)) (do (do (do c ol) o1) o2) /\ 
@@ -850,16 +892,17 @@ let comm_inter_base_left (l a b c:concrete_st) (o1 o2 ob ol:op_t)
   let k = get_key ob in
   let l' = sel l k in let a' = sel a k in let b' = sel b k in let c' = sel c k in
   if get_key o2 = get_key o1 && get_key o1 = k then 
-    comm_inter_base_left_s l' a' b' c' (get_op_s o1) (get_op_s o2) (get_op_s ob) (get_op_s ol)
+    comm_inter_base_left_v l' a' b' c' (get_op_v o1) (get_op_v o2) (get_op_v ob) (get_op_v ol)
   else comm_inter_base_left_ne l a b c o1 o2 ob ol
 
-val comm_inter_right_s (l a b c:concrete_st_s) (o1 o2 ob ol o:op_s)
-  : Lemma (requires rc_s ob ol <> Either /\ 
+val comm_inter_right_v (l a b c:concrete_st_v) (o1 o2 ob ol o:op_v)
+  : Lemma (requires Either? (rc_v o1 o2) /\ Fst_then_snd? (rc_v ob ol) /\ 
                     distinct_ops o1 o2 /\ distinct_ops o1 ob /\ distinct_ops o1 ol /\ distinct_ops o1 o /\ distinct_ops o2 ob /\ 
                     distinct_ops o2 ol /\ distinct_ops o2 o /\ distinct_ops ob ol /\ distinct_ops ob o /\ distinct_ops ol o /\
                     get_rid o <> get_rid ol (*o,ol must be concurrent*) /\
-                    eq_s (merge_s (do_s l ol) (do_s (do_s a ol) o1) (do_s (do_s (do_s b ob) ol) o2)) (do_s (do_s (do_s (do_s c ob) ol) o1) o2))
-          (ensures eq_s (merge_s (do_s l ol) (do_s (do_s a ol) o1) (do_s (do_s (do_s (do_s b o) ob) ol) o2)) (do_s (do_s (do_s (do_s (do_s c o) ob) ol) o1) o2))
+                    ((~ (commutes_with_v o ob)) \/ Fst_then_snd? (rc_v o ol)) /\
+                    eq_v (merge_v (do_v l ol) (do_v (do_v a ol) o1) (do_v (do_v (do_v b ob) ol) o2)) (do_v (do_v (do_v (do_v c ob) ol) o1) o2))
+          (ensures eq_v (merge_v (do_v l ol) (do_v (do_v a ol) o1) (do_v (do_v (do_v (do_v b o) ob) ol) o2)) (do_v (do_v (do_v (do_v (do_v c o) ob) ol) o1) o2))
           
 val comm_inter_right_ne (l a b c:concrete_st) (o1 o2 ob ol o:op_t)
   : Lemma (requires Either? (rc o1 o2) /\ Fst_then_snd? (rc ob ol) /\ 
@@ -881,19 +924,20 @@ let comm_inter_right (l a b c:concrete_st) (o1 o2 ob ol o:op_t)
                     ((~ (commutes_with o ob)) \/ Fst_then_snd? (rc o ol)) /\
                     eq (merge (do l ol) (do (do a ol) o1) (do (do (do b ob) ol) o2)) (do (do (do (do c ob) ol) o1) o2))
           (ensures eq (merge (do l ol) (do (do a ol) o1) (do (do (do (do b o) ob) ol) o2)) (do (do (do (do (do c o) ob) ol) o1) o2)) =
-    let k = get_key o in
+  let k = get_key o in
   let l' = sel l k in let a' = sel a k in let b' = sel b k in let c' = sel c k in
   if get_key o2 = get_key o1 && get_key o1 = k then 
-    comm_inter_right_s l' a' b' c' (get_op_s o1) (get_op_s o2) (get_op_s ob) (get_op_s ol) (get_op_s o)
+    comm_inter_right_v l' a' b' c' (get_op_v o1) (get_op_v o2) (get_op_v ob) (get_op_v ol) (get_op_v o)
   else comm_inter_right_ne l a b c o1 o2 ob ol o
 
-val comm_inter_left_s (l a b c:concrete_st_s) (o1 o2 ob ol o:op_s)
-  : Lemma (requires rc_s ob ol <> Either /\ 
+val comm_inter_left_v (l a b c:concrete_st_v) (o1 o2 ob ol o:op_v)
+  : Lemma (requires Either? (rc_v o1 o2) /\ Fst_then_snd? (rc_v ob ol) /\ 
                     distinct_ops o1 o2 /\ distinct_ops o1 ob /\ distinct_ops o1 ol /\ distinct_ops o1 o /\ distinct_ops o2 ob /\ 
                     distinct_ops o2 ol /\ distinct_ops o2 o /\ distinct_ops ob ol /\ distinct_ops ob o /\ distinct_ops ol o /\
                     get_rid o <> get_rid ol (*o,ol must be concurrent*) /\
-                    eq_s (merge_s (do_s l ol) (do_s (do_s (do_s a ob) ol) o1) (do_s (do_s b ol) o2)) (do_s (do_s (do_s (do_s c ob) ol) o1) o2))
-          (ensures eq_s (merge_s (do_s l ol) (do_s (do_s (do_s (do_s a o) ob) ol) o1) (do_s (do_s b ol) o2)) (do_s (do_s (do_s (do_s (do_s c o) ob) ol) o1) o2))
+                    ((~ (commutes_with_v o ob)) \/ Fst_then_snd? (rc_v o ol)) /\
+                    eq_v (merge_v (do_v l ol) (do_v (do_v (do_v a ob) ol) o1) (do_v (do_v b ol) o2)) (do_v (do_v (do_v (do_v c ob) ol) o1) o2))
+          (ensures eq_v (merge_v (do_v l ol) (do_v (do_v (do_v (do_v a o) ob) ol) o1) (do_v (do_v b ol) o2)) (do_v (do_v (do_v (do_v (do_v c o) ob) ol) o1) o2))
           
 val comm_inter_left_ne (l a b c:concrete_st) (o1 o2 ob ol o:op_t)
   : Lemma (requires Either? (rc o1 o2) /\ Fst_then_snd? (rc ob ol) /\ 
@@ -915,17 +959,17 @@ let comm_inter_left (l a b c:concrete_st) (o1 o2 ob ol o:op_t)
                     ((~ (commutes_with o ob)) \/ Fst_then_snd? (rc o ol)) /\
                     eq (merge (do l ol) (do (do (do a ob) ol) o1) (do (do b ol) o2)) (do (do (do (do c ob) ol) o1) o2))
           (ensures eq (merge (do l ol) (do (do (do (do a o) ob) ol) o1) (do (do b ol) o2)) (do (do (do (do (do c o) ob) ol) o1) o2)) =
-    let k = get_key o in
+  let k = get_key o in
   let l' = sel l k in let a' = sel a k in let b' = sel b k in let c' = sel c k in
   if get_key o2 = get_key o1 && get_key o1 = k then 
-    comm_inter_left_s l' a' b' c' (get_op_s o1) (get_op_s o2) (get_op_s ob) (get_op_s ol) (get_op_s o)
+    comm_inter_left_v l' a' b' c' (get_op_v o1) (get_op_v o2) (get_op_v ob) (get_op_v ol) (get_op_v o)
   else comm_inter_left_ne l a b c o1 o2 ob ol o
 
-val comm_inter_lca_s (l a b c:concrete_st_s) (o1 o2 ol:op_s)
-  : Lemma (requires distinct_ops o1 o2 /\ distinct_ops o1 ol /\ distinct_ops ol o2 /\
-                    (exists o'. rc_s o' ol <> Either) /\
-                    eq_s (merge_s l (do_s a o1) (do_s b o2)) (do_s (do_s c o1) o2))
-          (ensures eq_s (merge_s (do_s l ol) (do_s (do_s a ol) o1) (do_s (do_s b ol) o2)) (do_s (do_s (do_s c ol) o1) o2))
+val comm_inter_lca_v (l a b c:concrete_st_v) (o1 o2 ol:op_v)
+  : Lemma (requires Either? (rc_v o1 o2) /\ distinct_ops o1 o2 /\ distinct_ops o1 ol /\ distinct_ops ol o2 /\
+                    (exists o'. Fst_then_snd? (rc_v o' ol)) /\
+                    eq_v (merge_v l (do_v a o1) (do_v b o2)) (do_v (do_v c o1) o2))
+          (ensures eq_v (merge_v (do_v l ol) (do_v (do_v a ol) o1) (do_v (do_v b ol) o2)) (do_v (do_v (do_v c ol) o1) o2))
 
 val comm_inter_lca_ne (l a b c:concrete_st) (o1 o2 ol:op_t)
   : Lemma (requires Either? (rc o1 o2) /\ 
@@ -944,5 +988,5 @@ let comm_inter_lca (l a b c:concrete_st) (o1 o2 ol:op_t)
   let k = get_key ol in
   let l' = sel l k in let a' = sel a k in let b' = sel b k in let c' = sel c k in
   if get_key o2 = get_key o1 && get_key o1 = k then 
-    comm_inter_lca_s l' a' b' c' (get_op_s o1) (get_op_s o2) (get_op_s ol)
+    comm_inter_lca_v l' a' b' c' (get_op_v o1) (get_op_v o2) (get_op_v ol)
   else comm_inter_lca_ne l a b c o1 o2 ol
