mrdts-new/Set-wins_map/App.fst
@@ -12,7 +12,7 @@ type concrete_st = S.t (pos & (nat & nat)) //set of (timestamp, (key, value))
 let init_st : concrete_st = S.empty
   
 // equivalence between 2 concrete states
-let eq (a b:concrete_st) = S.equal a b
+let eq (a b:concrete_st) = a == b
 
 let symmetric (a b:concrete_st) 
   : Lemma (requires eq a b)
@@ -59,6 +59,7 @@ let merge (l a b:concrete_st) : concrete_st =
 
 /////////////////////////////////////////////////////////////////////////////
 
+#set-options "--z3rlimit 300 --ifuel 3"
 let rc_non_comm_help1 (o1 o2:op_t)
   : Lemma (requires distinct_ops o1 o2)
           (ensures ((Set? (snd (snd o1)) /\ Del? (snd (snd o2)) /\ get_key o1 = get_key o2) ==> ~ (eq (do (do init_st o1) o2) (do (do init_st o2) o1)))) = ()
@@ -77,16 +78,17 @@ let no_rc_chain (o1 o2 o3:op_t)
   : Lemma (requires distinct_ops o1 o2 /\ distinct_ops o2 o3)
           (ensures ~ (Fst_then_snd? (rc o1 o2) /\ Fst_then_snd? (rc o2 o3))) = ()
 
-let cond_comm_base (s:concrete_st) (o1 o2:op_t) (o3:op_t{distinct_ops o1 o2 /\ distinct_ops o1 o3 /\ distinct_ops o2 o3})
-    : (b:bool{(Fst_then_snd? (rc o1 o2) /\ ~ (Either? (rc o2 o3))) ==> eq (do (do (do s o1) o2) o3) (do (do (do s o2) o1) o3)}) = 
-    if Del? (snd (snd o3)) && get_key o1 = get_key o3 then true else false
+let cond_comm_base (s:concrete_st) (o1 o2 o3:op_t) 
+  : Lemma (requires distinct_ops o1 o2 /\ distinct_ops o2 o3 /\ distinct_ops o1 o3 /\
+                    Fst_then_snd? (rc o1 o2) /\ ~ (Either? (rc o2 o3)))
+          (ensures eq (do (do (do s o1) o2) o3) (do (do (do s o2) o1) o3)) = ()
 
-#push-options "--z3rlimit 50 --max_ifuel 3"
 let cond_comm_ind (s:concrete_st) (o1 o2 o3 o:op_t) (l:seq op_t)
-  : Lemma (requires distinct_ops o1 o2 /\ distinct_ops o1 o3 /\ distinct_ops o2 o3 /\ cond_comm_base s o1 o2 o3 /\
+  : Lemma (requires distinct_ops o1 o2 /\ distinct_ops o1 o3 /\ distinct_ops o2 o3 /\ 
+                    Fst_then_snd? (rc o1 o2) /\ ~ (Either? (rc o2 o3)) /\
                     eq (do (apply_log (do (do s o1) o2) l) o3) (do (apply_log (do (do s o2) o1) l) o3))
           (ensures eq (do (do (apply_log (do (do s o1) o2) l) o) o3) (do (do (apply_log (do (do s o2) o1) l) o) o3)) = ()
- 
+          
 /////////////////////////////////////////////////////////////////////////////
 // Merge commutativity
 let merge_comm (l a b:concrete_st)
@@ -195,8 +197,8 @@ let one_op_inter_base_left (l a b c:concrete_st) (o2 ob ol:op_t)
                     eq (merge (do l ol) (do a ol) (do (do b ol) o2)) (do (do c ol) o2) /\
                     (Fst_then_snd? (rc ob o2) ==> eq (merge l (do a o2) (do b ob)) (do (merge l a (do b ob)) o2)) /\ //***EXTRA***
                     eq (merge l a (do b o2)) (do c o2) /\
-                    eq (merge l (do a ol) (do b ob)) (do (do c ob) ol) /\ //***EXTRA***
-                    eq (merge l (do (do a ob) ol) (do b ol)) (do (do c ob) ol)) //***EXTRA***
+                    eq (merge l (do a ob) (do b o2)) (do (do c ob) o2) /\ //EXTRA!! 
+                    eq (merge l (do a ob) (do b ol)) (do (do c ob) ol)) //***EXTRA***
           (ensures eq (merge (do l ol) (do (do a ob) ol) (do (do b ol) o2)) (do (do (do c ob) ol) o2)) = ()
 
 let one_op_inter_right (l a b c:concrete_st) (o2 ob ol o:op_t) 
