interface/Map_extended.fst
@@ -108,5 +108,5 @@ let equal (#key:eqtype) (#value:Type) (m1:t key value) (m2:t key value) : Type0 
     S.equal m1.domain m2.domain
 
 let lemma_equal_intro #key #value m1 m2 = ()
-let lemma_equal_intro' #key #value m1 m2 = ()
 let lemma_equal_elim #key #value m1 m2  = ()
+let lemma_equal_intro' #key #value m1 m2 = ()
